@prefix owl: <http://www.w3.org/2002/07/owl#> .
@prefix rdfs: <http://www.w3.org/2000/01/rdf-schema#> .
@prefix xsd: <http://www.w3.org/2001/XMLSchema#> .
@prefix ns0: <https://w3id.org/iot-tta#> .
@prefix ns1: <http://swrl.stanford.edu/ontologies/3.3/swrla.owl#> .
@prefix ns2: <http://www.w3.org/2003/11/swrl#> .
@prefix dcterms: <http://purl.org/dc/terms/> .
@prefix voaf: <http://purl.org/vocommons/voaf#> .
@prefix vann: <http://purl.org/vocab/vann/> .

## Ontology metadata here 
<https://w3id.org/iot-tta>
  a owl:Ontology, voaf:Vocabulary ;
  owl:versionIRI <https://tudorliv.github.io/IoT-TTA/IIoT_v1.4.ttl>;
  owl:versionInfo "Version 1.4" ;
  dcterms:creator https://scholar.google.com/citations?user=WQu1J74AAAAJ&hl=en ;
  vann:preferredNamespacePrefix "iot-tta";
  vann:preferredNamespaceUri <https://w3id.org/iot-tta#> ;
  dcterms:contributor https://scholar.google.com/citations?user=fzNnkykAAAAJ&hl=en; 
                      https://scholar.google.com/citations?user=SpVRxaYAAAAJ&hl=en; 
                      https://scholar.google.com/citations?user=VREZXUYAAAAJ&hl=en;
                      https://www.colorado.edu/cmci/2021/05/03/class-2021-clark-mousaw;                      
  dcterms:issued "2022-08-27"^^xsd:date ;
  dcterms:modified "2022-09-02"^^xsd:date ;
  dcterms:title "Ontology for Internet of Things Technologies, Tools, and Applications"@en ;
  dcterms:description " The Internet of Things taxonomy is extended with semantic ontologies for IoT layers, containing classes, properties, individuals, and rules specific to IoT technologies, tools, and applications."@en;
  .
  



## Ontology properties 

<http://swrl.stanford.edu/ontologies/3.3/swrla.owl#isRuleEnabled> a owl:AnnotationProperty .
<https://w3id.org/iot-tta#dealing_with_sensitive_data>
  a owl:ObjectProperty ;
  rdfs:label "Dealing with sensitive data";
  rdfs:domain <https://w3id.org/iot-tta#SCADA> ;
  rdfs:range <https://w3id.org/iot-tta#SCADA_solution> ;
  rdfs:comment "Dealing_with_sensitive_data (Object property): SCADA solutions are proper practices for systems dealing with sensitive data"@en .

<https://w3id.org/iot-tta#developEdgeSecurity>
  a owl:ObjectProperty ;
  rdfs:domain <https://w3id.org/iot-tta#Edge_application> ;
  rdfs:range <https://w3id.org/iot-tta#Blockchain_solution> ;
  rdfs:comment "DevelopEdgeSecurity (Object property): develops solutions for edge applications using Blockchain capabilities"@en .

<https://w3id.org/iot-tta#Lack_security_measure>
  a owl:ObjectProperty ;
  rdfs:domain <https://w3id.org/iot-tta#SCADA_common_protocol> ;
  rdfs:range <https://w3id.org/iot-tta#SCADA_problem> ;
  rdfs:comment "Lack_security_measure (Object property): The SCADA common protocols such as Modbus and BACnet lack the built-in security measures"@en .

<https://w3id.org/iot-tta#Protocols_were_layered>
  a owl:ObjectProperty ;
  rdfs:domain <https://w3id.org/iot-tta#SCADA_common_protocol> ;
  rdfs:range <https://w3id.org/iot-tta#SCADA_today_protocol> ;
  rdfs:comment "Protocols_were_layered (Object property): SCADA common protocols, such as Modbus and BACnet, were layered into Ethernet and TCP/IP"@en .

<https://w3id.org/iot-tta#SCADA_hasCapability>
  a owl:ObjectProperty ;
  rdfs:domain <https://w3id.org/iot-tta#SCADA> ;
  rdfs:range <https://w3id.org/iot-tta#SCADA_capability> ;
  rdfs:comment "SCADA_hasCapability (Object property): SCADA systems provide  capabilities for industrial systems"@en .

<https://w3id.org/iot-tta#Support_communication>
  a owl:ObjectProperty ;
  rdfs:domain <https://w3id.org/iot-tta#SCADA_today_protocol> ;
  rdfs:range <https://w3id.org/iot-tta#SCADA_capability> ;
  rdfs:comment "Support_communication (Object property): SCADA systems perform communication with industrial systems in distributed architectures"@en .

<https://w3id.org/iot-tta#authentication>
  a owl:ObjectProperty ;
  rdfs:domain <https://w3id.org/iot-tta#MQTT> ;
  rdfs:range <https://w3id.org/iot-tta#Asymmetric_public_keys>, <https://w3id.org/iot-tta#JSON_Web_Token> ;
  rdfs:comment "authentication (Object property): the MQTT and HTTP bridges use authentication with asymmetric public keys and JSON Web tokens"@en .

<https://w3id.org/iot-tta#best_Practices>
  a owl:ObjectProperty ;
  rdfs:domain <https://w3id.org/iot-tta#Edge_security> ;
  rdfs:range <https://w3id.org/iot-tta#Edge_application> ;
  rdfs:comment "best_Practices (Object property): defines the best practices for the edge security problems using Blockchain solutions"@en .

<https://w3id.org/iot-tta#challenge>
  a owl:ObjectProperty ;
  rdfs:domain <https://w3id.org/iot-tta#Blockchain> ;
  rdfs:range <https://w3id.org/iot-tta#Blockchain_problem> ;
  rdfs:comment "challenge (Object property): Blockchain technology comes with some challenges to implementation"@en .

<https://w3id.org/iot-tta#countermeasure>
  a owl:ObjectProperty ;
  rdfs:domain <https://w3id.org/iot-tta#SCADA_problem> ;
  rdfs:range <https://w3id.org/iot-tta#SCADA_solution> ;
  rdfs:comment "countermeasure (Object property): SCADA solutions represent countermeasure against threats generated by SCADA security problems"@en .

<https://w3id.org/iot-tta#data_transfer>
  a owl:ObjectProperty ;
  rdfs:domain <https://w3id.org/iot-tta#MQTT> ;
  rdfs:range <https://w3id.org/iot-tta#Device> ;
  rdfs:comment "data_transfer (Object property): an MQTT protocol transfers data provided by sensors"@en .

<https://w3id.org/iot-tta#flow_services>
  a owl:ObjectProperty ;
  rdfs:domain <https://w3id.org/iot-tta#Particle_Photon> ;
  rdfs:range <https://w3id.org/iot-tta#Subscriber> ;
  rdfs:comment "flow_services: Object property that ensures the flows and services from Particle Photon to the subscriber (Thingspeak)"@en .

<https://w3id.org/iot-tta#hasAlgorithm>
  a owl:ObjectProperty ;
  rdfs:domain <https://w3id.org/iot-tta#Gateway> ;
  rdfs:range <https://w3id.org/iot-tta#Analytics>, <https://w3id.org/iot-tta#Machine_Learning> ;
  rdfs:comment "hasAlgorithm (Object property): Gateway devices provide real-time analytics or machine learning algorithms, in edge computing"@en .

<https://w3id.org/iot-tta#hasCapability>
  a owl:ObjectProperty ;
  rdfs:subPropertyOf owl:topObjectProperty ;
  rdfs:domain <https://w3id.org/iot-tta#Tool> ;
  rdfs:range <https://w3id.org/iot-tta#BigData_capability> ;
  rdfs:comment "hasCapability (Object property): tool that provides capabilities for big data processing in distributed systems"@en .

<https://w3id.org/iot-tta#hasElement>
  a owl:ObjectProperty ;
  rdfs:domain <https://w3id.org/iot-tta#Andrew> ;
  rdfs:range <https://w3id.org/iot-tta#Transducer> ;
  rdfs:comment "hasElement (Object property): Sensor Andrew - sharing of transducers. There are two types of transducers: sensors and actuators."@en .

<https://w3id.org/iot-tta#hasFunctionality>
  a owl:ObjectProperty ;
  rdfs:domain <https://w3id.org/iot-tta#Data_center> ;
  rdfs:range <https://w3id.org/iot-tta#Cloud_service> ;
  rdfs:comment "hasFunctionality (Object property): a data center offers cloud services (as functionality)"@en .

<https://w3id.org/iot-tta#hasProblem>
  a owl:ObjectProperty ;
  rdfs:domain <https://w3id.org/iot-tta#Blockchain> ;
  rdfs:range <https://w3id.org/iot-tta#Blockchain_problem> ;
  rdfs:comment "hasProblem (Object property): Blockchain technology has some problems"@en .

<https://w3id.org/iot-tta#hasSecurity_problem>
  a owl:ObjectProperty ;
  rdfs:domain <https://w3id.org/iot-tta#Blockchain> ;
  rdfs:range <https://w3id.org/iot-tta#Blockchain_solution> ;
  rdfs:comment "hasSecurity_problem (Object property): security problems in Blockchain technology"@en .

<https://w3id.org/iot-tta#hasService>
  a owl:ObjectProperty, owl:FunctionalProperty ;
  rdfs:domain <https://w3id.org/iot-tta#Data_center> ;
  rdfs:range <https://w3id.org/iot-tta#Cloud_service> ;
  rdfs:comment "hasService (Object property): specifies cloud services provided by data centers"@en .

<https://w3id.org/iot-tta#hasSolution>
  a owl:ObjectProperty ;
  rdfs:domain <https://w3id.org/iot-tta#Blockchain_problem> ;
  rdfs:range <https://w3id.org/iot-tta#Blockchain_solution> ;
  rdfs:comment "hasSolution (Object property): solutions for Blockchain problems"@en .

<https://w3id.org/iot-tta#hasTechnology>
  a owl:ObjectProperty ;
  rdfs:domain <https://w3id.org/iot-tta#Edge_application> ;
  rdfs:range <https://w3id.org/iot-tta#Edge_technology> ;
  rdfs:comment "hasTechnology (Object property): the technology used in edge computing applications"@en .

<https://w3id.org/iot-tta#hasTool>
  a owl:ObjectProperty ;
  rdfs:label "Has tool";
  rdfs:domain <https://w3id.org/iot-tta#Technology> ;
  rdfs:range <https://w3id.org/iot-tta#Tool> ;
  rdfs:comment "hasTool (Object property): a tool used for the implementation of a technology"@en .

<https://w3id.org/iot-tta#has_SecuritySolution>
  a owl:ObjectProperty ;
  rdfs:domain <https://w3id.org/iot-tta#Edge_security> ;
  rdfs:range <https://w3id.org/iot-tta#Blockchain_solution> ;
  rdfs:comment "has_SecuritySolution (Object property): defines the best practices based on Blockchain solutions for edge security problems"@en .

<https://w3id.org/iot-tta#heat>
  a owl:ObjectProperty ;
  rdfs:domain <https://w3id.org/iot-tta#RTD_sensor> ;
  rdfs:range <https://w3id.org/iot-tta#Industrial_oven> ;
  rdfs:comment "heat (Object property): RTD sensors provide heat for some industrial ovens"@en .

<https://w3id.org/iot-tta#isApplied>
  a owl:ObjectProperty ;
  rdfs:domain <https://w3id.org/iot-tta#Tool> ;
  rdfs:range <https://w3id.org/iot-tta#Computer_cluster> ;
  rdfs:comment "isApplied (Object property): a tool used for computer clusters"@en .

<https://w3id.org/iot-tta#isConnectedBy>
  a owl:ObjectProperty ;
  rdfs:domain <https://w3id.org/iot-tta#Processing_Board> ;
  rdfs:range <https://w3id.org/iot-tta#Smart_Product> ;
  rdfs:comment "isConnectedBy (Object property): modules with sensors or actuators connect processing boards with smart products"@en .

<https://w3id.org/iot-tta#isIdentified>
  a owl:ObjectProperty ;
  rdfs:domain <https://w3id.org/iot-tta#Passive_things> ;
  rdfs:range <https://w3id.org/iot-tta#BLE>, <https://w3id.org/iot-tta#NFC_tag>, <https://w3id.org/iot-tta#Optical_tag>, <https://w3id.org/iot-tta#RFID_tag> ;
  rdfs:comment "isIdentified (Object property): passive things are identified by protocols such as NFC tags, optical tags, BLE, RFID tag, etc."@en .

<https://w3id.org/iot-tta#isManagedBy>
  a owl:ObjectProperty ;
  rdfs:domain <https://w3id.org/iot-tta#Smart_Product> ;
  rdfs:range <https://w3id.org/iot-tta#Programming_Language>, <https://w3id.org/iot-tta#Web_Technology> ;
  rdfs:comment "isManagedBy (Object property): Smart products are managed using Web technologies and software platforms."@en .

<https://w3id.org/iot-tta#isPartOf>
  a owl:ObjectProperty ;
  rdfs:domain <https://w3id.org/iot-tta#PLC>, <https://w3id.org/iot-tta#SCADA> ;
  rdfs:range <https://w3id.org/iot-tta#ICS> ;
  rdfs:comment "isPartOf (Object property):  PLC/SCADA is part of ICS (Industrial Control Systems)"@en .

<https://w3id.org/iot-tta#isProcessed>
  a owl:ObjectProperty ;
  rdfs:domain <https://w3id.org/iot-tta#BigData> ;
  rdfs:range <https://w3id.org/iot-tta#BigData_capability> ;
  rdfs:comment "isProcessed (Object property): the big data relies on distributed processing and storing, data analytics, and machine learning"@en .

<https://w3id.org/iot-tta#isRepresentationOf>
  a owl:ObjectProperty ;
  rdfs:domain <https://w3id.org/iot-tta#Digital_twin> ;
  rdfs:range <https://w3id.org/iot-tta#Smart_Product> ;
  rdfs:comment "isRepresentationOf (Object property): A digital twin from the cloud is a software representation of a smart product"@en .

<https://w3id.org/iot-tta#isToolFor>
  a owl:ObjectProperty ;
  rdfs:domain <https://w3id.org/iot-tta#Tool> ;
  rdfs:range <https://w3id.org/iot-tta#Technology> ;
  rdfs:comment "isToolFor (Object property): tool for distributed computing technologies"@en .

<https://w3id.org/iot-tta#isUsedBy>
  a owl:ObjectProperty ;
  rdfs:domain <https://w3id.org/iot-tta#Tool> ;
  rdfs:range <https://w3id.org/iot-tta#Technology> ;
  rdfs:comment "isUsedBy (Object property): a tool used by a particular technology"@en .

<https://w3id.org/iot-tta#login>
  a owl:ObjectProperty ;
  rdfs:domain <https://w3id.org/iot-tta#Mobile_node> ;
  rdfs:range <https://w3id.org/iot-tta#Gateway> ;
  rdfs:comment "login (Object property): In a wireless sensor network, a mobile node logins with a password using a gateway and Publish-Subscribe service."@en .

<https://w3id.org/iot-tta#manages>
  a owl:ObjectProperty ;
  rdfs:domain <https://w3id.org/iot-tta#Gateway> ;
  rdfs:range <https://w3id.org/iot-tta#Sensor_Actuator> ;
  rdfs:comment "manages (Object property): Gateways manage the data from multiple devices and send them to the cloud"@en .

<https://w3id.org/iot-tta#read>
  a owl:ObjectProperty ;
  rdfs:domain <https://w3id.org/iot-tta#Flow> ;
  rdfs:range <https://w3id.org/iot-tta#Firmware> ;
  rdfs:comment "read (Object property): A firmware program reads the D0 value of the 3V3 pin, in an application with a  Particle Photon that publishes messages using a Webhook."@en .

<https://w3id.org/iot-tta#regulationTemperature>
  a owl:ObjectProperty ;
  rdfs:domain <https://w3id.org/iot-tta#RTD_sensor> ;
  rdfs:range <https://w3id.org/iot-tta#Industrial_oven> ;
  rdfs:comment "regulationTemperature (Object property): regulation of the RTD sensors’ temperature for an industrial oven"@en .

<https://w3id.org/iot-tta#request>
  a owl:ObjectProperty ;
  rdfs:domain <https://w3id.org/iot-tta#Particle_cloud> ;
  rdfs:range <https://w3id.org/iot-tta#Subscriber> ;
  rdfs:comment "request (Object property): Particle cloud service will forward messages with values “1” and “0” to Thingspeak as a subscriber. A Webhook (a new HTTP request to Thingspeak) will result after passing values to the Particle cloud."@en .

<https://w3id.org/iot-tta#requires>
  a owl:ObjectProperty ;
  rdfs:domain <https://w3id.org/iot-tta#BigData_app> ;
  rdfs:range <https://w3id.org/iot-tta#BigData_capability> ;
  rdfs:comment "requires (Object property): Applications with Big Data require Big data capabilities - distributed processing and storing, etc."@en .

<https://w3id.org/iot-tta#send>
  a owl:ObjectProperty ;
  rdfs:domain <https://w3id.org/iot-tta#Firmware> ;
  rdfs:range <https://w3id.org/iot-tta#Particle_cloud> ;
  rdfs:comment "send (Object property): A firmware program that reads the D0 value every 30 seconds, calls the function Particle.publish() with one of the values “0” or “1” that is sent to the Particle cloud."@en .

<https://w3id.org/iot-tta#supporting_tool>
  a owl:ObjectProperty ;
  rdfs:domain <https://w3id.org/iot-tta#Edge_application> ;
  rdfs:range <https://w3id.org/iot-tta#Tool> ;
  rdfs:comment "supporting_tool (Object property): tools for edge computing applications"@en .

<https://w3id.org/iot-tta#threats_to_data_security>
  a owl:ObjectProperty ;
  rdfs:domain <https://w3id.org/iot-tta#SCADA> ;
  rdfs:range <https://w3id.org/iot-tta#SCADA_problem> ;
  rdfs:comment "threats_to_data_security (Object property): SCADA protocols require an adequate defense against data security threats"@en .

<https://w3id.org/iot-tta#useAlgorithm>
  a owl:ObjectProperty ;
  rdfs:subPropertyOf owl:topObjectProperty ;
  rdfs:domain <https://w3id.org/iot-tta#Data_center> ;
  rdfs:range <https://w3id.org/iot-tta#Data_center> ;
  rdfs:comment "useAlgorithm (Object property): algorithms used in data centers"@en .

<https://w3id.org/iot-tta#useProgramming>
  a owl:ObjectProperty ;
  rdfs:subPropertyOf owl:topObjectProperty ;
  rdfs:domain <https://w3id.org/iot-tta#Tool> ;
  rdfs:range <https://w3id.org/iot-tta#Tool> ;
  rdfs:comment "useProgramming (Object property): defines the programming model used by tools for computer clusters"@en .

<https://w3id.org/iot-tta#wire>
  a owl:ObjectProperty ;
  rdfs:domain <https://w3id.org/iot-tta#Particle_Photon> ;
  rdfs:range <https://w3id.org/iot-tta#Flow> ;
  rdfs:comment "wire (Object property): When the wire of a Particle Photon is connected, the Photon will send the value “1”, but if the wire is disconnected, the Photon will send the value “0”."@en .

<https://w3id.org/iot-tta#FireFly_nodes>
  a owl:DatatypeProperty ;
  rdfs:domain <https://w3id.org/iot-tta#Wireless_sensor_network>, [
    a owl:Restriction ;
    owl:onProperty <https://w3id.org/iot-tta#FireFly_nodes> ;
    owl:someValuesFrom [
      a rdfs:Datatype ;
      owl:onDatatype xsd:integer ;
      owl:withRestrictions (
       _:genid3
       _:genid5
     )
    ]
  ] ;
  rdfs:range xsd:integer ;
  rdfs:comment "FireFly_nodes (Data property): in a FireFly wireless sensor network, each gateway is set to manage between 20 and 32 network nodes"@en .

<https://w3id.org/iot-tta#MicroSD_card>
  a owl:DatatypeProperty ;
  rdfs:subPropertyOf owl:topDataProperty ;
  rdfs:domain <https://w3id.org/iot-tta#Raspberyy_Pi_4B>, [
    a owl:Restriction ;
    owl:onProperty <https://w3id.org/iot-tta#MicroSD_card> ;
    owl:someValuesFrom [
      a rdfs:Datatype ;
      owl:onDatatype xsd:double ;
      owl:withRestrictions ( _:genid9 )
    ]
  ] ;
  rdfs:range xsd:double ;
  rdfs:comment "MicroSD_card (Data property): setting up Raspberry Pi 4 Model B requires a microSD card with a capacity of at least 8GB"@en .

<https://w3id.org/iot-tta#Password_mobile_node>
  a owl:DatatypeProperty ;
  rdfs:domain <https://w3id.org/iot-tta#Wireless_sensor_network>, [
    a owl:Restriction ;
    owl:onProperty <https://w3id.org/iot-tta#Password_mobile_node> ;
    owl:hasValue "password"
  ] ;
  rdfs:range xsd:string ;
  rdfs:comment "Password_mobile_node (Data property): in a FireFly wireless sensor network, a mobile node logins with a password of at most 100 bytes"@en .

<https://w3id.org/iot-tta#Power_supply>
  a owl:DatatypeProperty ;
  rdfs:subPropertyOf owl:topDataProperty ;
  rdfs:domain <https://w3id.org/iot-tta#Raspberyy_Pi_4B>, [
    a owl:Restriction ;
    owl:onProperty <https://w3id.org/iot-tta#Power_supply> ;
    owl:someValuesFrom [
      a rdfs:Datatype ;
      owl:onDatatype xsd:float ;
      owl:withRestrictions ( _:genid14 )
    ]
  ] ;
  rdfs:range xsd:float ;
  rdfs:comment "Power_supply (Data property): Setting up Raspberry Pi 4 Model B requires a power supply that provides at least 3.0 amps"@en .

<https://w3id.org/iot-tta#RAM>
  a owl:DatatypeProperty ;
  rdfs:subPropertyOf owl:topDataProperty ;
  rdfs:domain <https://w3id.org/iot-tta#Raspberyy_Pi_4B>, [
    a owl:Restriction ;
    owl:onProperty <https://w3id.org/iot-tta#RAM> ;
    owl:someValuesFrom [
      a rdfs:Datatype ;
      owl:onDatatype xsd:integer ;
      owl:withRestrictions ( _:genid18 )
    ]
  ] ;
  rdfs:range xsd:integer ;
  rdfs:comment "RAM (Data property): setting up Raspberry Pi 4 Model B requires at least 2GB RAM for use as a desktop computer"@en .

<https://w3id.org/iot-tta#disconnect_timeout>
  a owl:DatatypeProperty ;
  rdfs:domain <https://w3id.org/iot-tta#Wireless_sensor_network>, [
    a owl:Restriction ;
    owl:onProperty <https://w3id.org/iot-tta#disconnect_timeout> ;
    owl:someValuesFrom [
      a rdfs:Datatype ;
      owl:onDatatype xsd:integer ;
      owl:withRestrictions ( _:genid22 )
    ]
  ] ;
  rdfs:range xsd:integer ;
  rdfs:comment "disconnect_timeout (Data property): in a FireFly wireless sensor network, the SAMPL messages require a disconnect timeout for replying to messages on the mobile device"@en .

<https://w3id.org/iot-tta#hasAccuracy>
  a owl:DatatypeProperty ;
  rdfs:domain <https://w3id.org/iot-tta#RTD_sensor>, [
    a owl:Restriction ;
    owl:onProperty <https://w3id.org/iot-tta#hasAccuracy> ;
    owl:someValuesFrom [
      a rdfs:Datatype ;
      owl:onDatatype xsd:float ;
      owl:withRestrictions (
       _:genid26
       _:genid28
     )
    ]
  ] ;
  rdfs:range xsd:float ;
  rdfs:comment "hasAccuracy (Data property): the accuracy provided by RTD sensors is between 0.1 and 1 °C"@en .

<https://w3id.org/iot-tta#hasTemperatureRange>
  a owl:DatatypeProperty ;
  rdfs:domain <https://w3id.org/iot-tta#Industrial_oven>, [
    a owl:Restriction ;
    owl:onProperty <https://w3id.org/iot-tta#hasTemperatureRange> ;
    owl:someValuesFrom [
      a rdfs:Datatype ;
      owl:onDatatype xsd:double ;
      owl:withRestrictions (
       _:genid32
       _:genid34
     )
    ]
  ] ;
  rdfs:range xsd:double ;
  rdfs:comment "hasTemperatureRange (Data property): an industrial oven for a production line that is heated to a very precise temperature range, between 500F and 510F"@en .

<https://w3id.org/iot-tta#hasTimeLimit>
  a owl:DatatypeProperty ;
  rdfs:domain <https://w3id.org/iot-tta#Firmware>, [
    a owl:Restriction ;
    owl:onProperty <https://w3id.org/iot-tta#hasTimeLimit> ;
    owl:someValuesFrom [
      a rdfs:Datatype ;
      owl:onDatatype xsd:integer ;
      owl:withRestrictions (
       _:genid38
       _:genid40
     )
    ]
  ] ;
  rdfs:range xsd:integer ;
  rdfs:comment "hasTimeLimit (Data property): A firmware program reads the D0 value of the 3V3 pin every 30 seconds, for an application with a  Particle Photon with a single resistor that publishes messages using a Webhook."@en .

<https://w3id.org/iot-tta#hasValueConnection>
  a owl:DatatypeProperty ;
  rdfs:domain <https://w3id.org/iot-tta#Flow>, [
    a owl:Restriction ;
    owl:onProperty <https://w3id.org/iot-tta#hasValueConnection> ;
    owl:someValuesFrom [
      a rdfs:Datatype ;
      owl:onDatatype xsd:integer ;
      owl:withRestrictions (
       _:genid44
       _:genid46
     )
    ]
  ] ;
  rdfs:range xsd:integer ;
  rdfs:comment "hasValueConnection (Data property): if the wire of a Particle Photon is connected, the Photon sends the value “1”"@en .

<https://w3id.org/iot-tta#languages_tools>
  a owl:DatatypeProperty ;
  rdfs:domain <https://w3id.org/iot-tta#PLC>, <https://w3id.org/iot-tta#Raspberry_Pi>, [
    a owl:Class ;
    owl:unionOf (
     _:genid49
     _:genid51
     _:genid53
     _:genid55
     _:genid57
     _:genid59
     _:genid61
   )
  ] ;
  rdfs:range xsd:string ;
  rdfs:comment "languages_tools (Data property): tools and programming languages used by hardware platforms like PLC and Raspberry Pi"@en .

<https://w3id.org/iot-tta#operating_system>
  a owl:DatatypeProperty ;
  rdfs:domain <https://w3id.org/iot-tta#Raspberry_Pi>, [
    a owl:Class ;
    owl:unionOf (
     _:genid64
     _:genid66
     _:genid68
     _:genid70
     _:genid72
     _:genid74
   )
  ] ;
  rdfs:range xsd:string ;
  rdfs:comment "operating_system (Data property): operating systems used by Raspberry Pi"@en .

<https://w3id.org/iot-tta#provideHeat>
  a owl:DatatypeProperty ;
  rdfs:domain <https://w3id.org/iot-tta#RTD_sensor>, [
    a owl:Restriction ;
    owl:onProperty <https://w3id.org/iot-tta#provideHeat> ;
    owl:someValuesFrom [
      a rdfs:Datatype ;
      owl:onDatatype xsd:double ;
      owl:withRestrictions (
       _:genid78
       _:genid80
     )
    ]
  ] ;
  rdfs:range xsd:double ;
  rdfs:comment "provideHeat (Data property): the RTD sensors provide heat between  -200 and 600 °C"@en .


## Ontology classes here 

<https://w3id.org/iot-tta#Blockchain_app>
  a owl:Class ;
  rdfs:subClassOf <https://w3id.org/iot-tta#Application> ;
  rdfs:comment "Blockchain can be used in IoT applications such as smart cities, e-health, agriculture, and IoT data processing."@en .

<https://w3id.org/iot-tta#AdaFruit>
  a owl:Class ;
  rdfs:subClassOf <https://w3id.org/iot-tta#MQTT_streams> ;
  rdfs:comment "Adafruit is a development board designed for Arduino, Raspberry Pi applications."@en .

<https://w3id.org/iot-tta#Adapter>
  a owl:Class ;
  rdfs:subClassOf <https://w3id.org/iot-tta#Gateway> ;
  rdfs:comment "Adapters are gateways to external hardware platforms like Arduino and Raspberry PI."@en .

<https://w3id.org/iot-tta#Algorithm>
  a owl:Class ;
  rdfs:subClassOf <https://w3id.org/iot-tta#Logic> ;
  rdfs:comment "Algorithms for data analytics, data mining, neural networks, firmware, and tools for machine learning."@en .

<https://w3id.org/iot-tta#Analytics>
  a owl:Class ;
  rdfs:subClassOf <https://w3id.org/iot-tta#Algorithm> ;
  rdfs:comment "Tools for data analysis: Spark, Hortonworks, Cloudera, MapR, Watson IoT"@en .

<https://w3id.org/iot-tta#Andrew>
  a owl:Class ;
  rdfs:subClassOf <https://w3id.org/iot-tta#Sensor_Actuator> ;
  rdfs:comment "Sensor Andrew - uniform access to heterogeneous devices; sharing of transducers; security and privacy, etc."@en .

<https://w3id.org/iot-tta#Application>
  a owl:Class ;
  rdfs:subClassOf <https://w3id.org/iot-tta#IoTLayers> ;
  rdfs:comment "\"Application\" represents a layer of the IoT architecture. Application layer ontology includes terms and semantic rules regarding Blockchain technology, SCADA systems, and security issues in cloud and edge computing."@en .

<https://w3id.org/iot-tta#Arduino>
  a owl:Class ;
  rdfs:subClassOf <https://w3id.org/iot-tta#Microcontroller> ;
  rdfs:comment "Arduino is a microcontroller based on the C++ language. Cosm and Nimbits are open platforms for storing sensor data on the Cloud."@en .

<https://w3id.org/iot-tta#Asymmetric_public_keys>
  a owl:Class ;
  rdfs:subClassOf <https://w3id.org/iot-tta#Cryptographic_system> ;
  rdfs:comment "The MQTT and HTTP bridges use authentication with asymmetric public key and JSON Web tokens, which increase device security."@en .

<https://w3id.org/iot-tta#BLE>
  a owl:Class ;
  rdfs:subClassOf <https://w3id.org/iot-tta#Protocol> ;
  rdfs:comment "BLE tags (Bluetooth Low Energy beacons) - protocols for small data exchanges are small Bluetooth hardware components that are used to locate people or objects."@en .

<https://w3id.org/iot-tta#BigData>
  a owl:Class ;
  rdfs:subClassOf <https://w3id.org/iot-tta#Technology> ;
  rdfs:comment "The data stream from IoT systems is processed using cloud computing, big data, and artificial intelligence algorithms."@en .

<https://w3id.org/iot-tta#BigData_app>
  a owl:Class ;
  rdfs:subClassOf <https://w3id.org/iot-tta#Application> ;
  rdfs:comment "Applications with Big Data - BigQuery, an enterprise data warehouse for large data that enables fast SQL queries"@en .

<https://w3id.org/iot-tta#BigData_capability>
  a owl:Class ;
  rdfs:subClassOf <https://w3id.org/iot-tta#BigData> ;
  rdfs:comment "Big data capabilities - distributed processing and storing, big data analytics, machine learning algorithms."@en .

<https://w3id.org/iot-tta#Blockchain>
  a owl:Class ;
  rdfs:subClassOf <https://w3id.org/iot-tta#Technology> ;
  rdfs:comment "Blockchain is a promising technology for securing IoT data over a network. Blockchain has distributed capabilities for processing transactions and tracking assets in a business network."@en .

<https://w3id.org/iot-tta#Blockchain_problem>
  a owl:Class ;
  rdfs:subClassOf <https://w3id.org/iot-tta#Blockchain> ;
  rdfs:comment "Blockchain problems: (a) Blockchain algorithm requires energy that IoT devices may not manage; (b) IoT devices continue to stream data while Blockchain throughput is limited; (c) Almost impossible to identify illegal Blockchain transaction; (d) Blockchain’s transparency feature brings privacy challenges for IoT customer, etc."@en .

<https://w3id.org/iot-tta#Blockchain_security>
  a owl:Class ;
  rdfs:subClassOf <https://w3id.org/iot-tta#Blockchain> ;
  rdfs:comment "Security for Blockchain is aimed at access control and securing communication between local IoT devices."@en .

<https://w3id.org/iot-tta#Blockchain_solution>
  a owl:Class ;
  rdfs:subClassOf <https://w3id.org/iot-tta#Blockchain> ;
  rdfs:comment "Solutions for Blockchain problems - improving data privacy, reducing latency in sending data, and adjusting the deficiencies of the edge implementation"@en .

<https://w3id.org/iot-tta#C>
  a owl:Class ;
  rdfs:subClassOf <https://w3id.org/iot-tta#Programming_Language> ;
  rdfs:comment "Embedded programming in C or C++ for IoT platforms like Arduino, Raspberry Pi, or Particle"@en .

<https://w3id.org/iot-tta#Capabilities>
  a owl:Class ;
  rdfs:subClassOf <https://w3id.org/iot-tta#IoTLayers> ;
  rdfs:comment "\"Capabilities\" represents a layer of the IoT architecture and includes device and data management, security, privacy, and ethics."@en .

<https://w3id.org/iot-tta#Cloud_service>
  a owl:Class ;
  rdfs:subClassOf <https://w3id.org/iot-tta#Support> ;
  rdfs:comment "Cloud services perform communications between devices, data gathering and processing."@en .

<https://w3id.org/iot-tta#Cloud_system>
  a owl:Class ;
  rdfs:subClassOf <https://w3id.org/iot-tta#Support> ;
  rdfs:comment "Cloud systems perform cloud computing. Instead of selling, cloud providers rent servers, storage space, databases, networks, software, analytics and business intelligence."@en .

<https://w3id.org/iot-tta#Cloudera>
  a owl:Class ;
  rdfs:subClassOf <https://w3id.org/iot-tta#Tool> ;
  rdfs:comment "Cloudera Data Platform (CDP) is a hybrid data platform for cloud computing, data analytics, and data management, offering performance, scalability, and security."@en .

<https://w3id.org/iot-tta#Cloudlet>
  a owl:Class ;
  rdfs:subClassOf <https://w3id.org/iot-tta#Support> ;
  rdfs:comment "Cloudlets are usually based on mini-center of servers with cloud services for mobile applications and edge computing. A cloudlet represents the middle level of a 3-level architecture: mobile device - cloudlet - cloud."@en .

<https://w3id.org/iot-tta#Computer_architecture>
  a owl:Class ;
  rdfs:subClassOf <https://w3id.org/iot-tta#Network> ;
  rdfs:comment "The Network class is defined as an aggregation of the three components: data transmission, control engineering, and computer architecture."@en .

<https://w3id.org/iot-tta#Computer_cluster>
  a owl:Class ;
  rdfs:subClassOf <https://w3id.org/iot-tta#Technology> ;
  rdfs:comment "A computer cluster is a set of computers that work together as a single system. Computer clusters have each node set to perform the same task, controlled and scheduled by software."@en .

<https://w3id.org/iot-tta#Control_System>
  a owl:Class ;
  rdfs:subClassOf <https://w3id.org/iot-tta#Purpose-built_Device> ;
  rdfs:comment "Examples of industrial control systems based on IoT technology are manufacturing processes, power grids, etc."@en .

<https://w3id.org/iot-tta#Control_engineering>
  a owl:Class ;
  rdfs:subClassOf <https://w3id.org/iot-tta#Network> ;
  rdfs:comment "The Network class is defined as an aggregation of the three components: data transmission, control engineering, and computer architecture."@en .

<https://w3id.org/iot-tta#Cryptographic_system>
  a owl:Class ;
  rdfs:subClassOf <https://w3id.org/iot-tta#Algorithm> ;
  rdfs:comment "A set of algorithms that convert plaintext to the ciphertext to encode or decode messages securely."@en .

<https://w3id.org/iot-tta#Data>
  a owl:Class ;
  rdfs:subClassOf <https://w3id.org/iot-tta#Support> ;
  rdfs:comment "Objects connected by sensors exchange data with other devices via the Internet."@en .

<https://w3id.org/iot-tta#Data_analysis>
  a owl:Class ;
  rdfs:subClassOf <https://w3id.org/iot-tta#Technology> ;
  rdfs:comment "Data analysis is a process of inspecting, pre-processing, and modeling data for knowledge discovery, complex data aggregation, visualization, and reporting. Data mining is a particular data analysis technique focused on statistical algorithms for prediction, classification, clustering, etc."@en .

<https://w3id.org/iot-tta#Data_center>
  a owl:Class ;
  rdfs:subClassOf <https://w3id.org/iot-tta#Support> ;
  rdfs:comment "A data center is a multicloud environment based on a network of computing, routers, switches, firewalls, storage systems, servers, and application-delivery controllers."@en .

<https://w3id.org/iot-tta#Data_transmission>
  a owl:Class ;
  rdfs:subClassOf <https://w3id.org/iot-tta#Network> ;
  rdfs:comment "The Network class is defined as an aggregation of the three components: data transmission, control engineering, and computer architecture."@en .

<https://w3id.org/iot-tta#Deep_learning>
  a owl:Class ;
  rdfs:subClassOf <https://w3id.org/iot-tta#Technology> ;
  rdfs:comment "Deep learning is a branch of machine learning that relies on multilayer neural networks. Deep learning offers a refined and optimized method of computation, using hidden layers of a neural network that often learns from large amounts of data. Deep learning technologies - Theano, Tensor Flow, CNTK, MXnet, Caffe on Spark"@en .

<https://w3id.org/iot-tta#Device>
  a owl:Class ;
  rdfs:subClassOf <https://w3id.org/iot-tta#IoTLayers> ;
  rdfs:comment "\"Device\" represents a layer of the IoT architecture. The device layer includes hardware platforms, connected products, technologies, tools, and functionalities."@en .

<https://w3id.org/iot-tta#Digital>
  a owl:Class ;
  rdfs:subClassOf <https://w3id.org/iot-tta#Device> ;
  rdfs:comment "Digital includes terms and tools about hardware platforms, logic, purpose-built devices, and smart products."@en .

<https://w3id.org/iot-tta#Digital_twin>
  a owl:Class ;
  rdfs:subClassOf <https://w3id.org/iot-tta#Web_Technology> ;
  rdfs:comment "A digital twin from the cloud can be associated with a device. The twin interacts with traditional browsers and with the backend device. The twin may be used to control or monitor the device."@en .

<https://w3id.org/iot-tta#Distributed_operating_system>
  a owl:Class ;
  rdfs:subClassOf <https://w3id.org/iot-tta#Support> ;
  rdfs:comment "A distributed operating system manages communication shared in a network of independent computers that possess their own memory unit and CPU. Ex: YARN, LOCUS, Mesos, etc."@en .

<https://w3id.org/iot-tta#Distributed_processing>
  a owl:Class ;
  rdfs:subClassOf <https://w3id.org/iot-tta#BigData_capability> ;
  rdfs:comment "Big data distributed processing - uploading significant volumes of data, data processing and analyzing, and distribution into the clustered database."@en .

<https://w3id.org/iot-tta#Distributed_storage>
  a owl:Class ;
  rdfs:subClassOf <https://w3id.org/iot-tta#BigData_capability> ;
  rdfs:comment "Big data distributed storage - stores and processes data on multiple machines, using services managed by cloud systems."@en .

<https://w3id.org/iot-tta#Distributed_system>
  a owl:Class ;
  rdfs:subClassOf <https://w3id.org/iot-tta#Support> ;
  rdfs:comment "The support layer is represented by distributed systems known as “cloud systems” that perform communications between devices, data gathering and processing. A distributed system has components located on different  computers from the network that communicate by passing messages."@en .

<https://w3id.org/iot-tta#Django>
  a owl:Class ;
  rdfs:subClassOf <https://w3id.org/iot-tta#Web_Technology> ;
  owl:disjointWith <https://w3id.org/iot-tta#Node> ;
  rdfs:comment "Software platforms (e.g., Python, Django, Node) and Web technologies are integrated with hardware components of the IoT systems. Django is a Python web framework used for the development of secure websites."@en .

<https://w3id.org/iot-tta#Drone>
  a owl:Class ;
  rdfs:subClassOf <https://w3id.org/iot-tta#Purpose-built_Device> ;
  rdfs:comment "Drones - flying IoT devices with full network connectivity capabilities."@en .

<https://w3id.org/iot-tta#Eddystone>
  a owl:Class ;
  rdfs:subClassOf <https://w3id.org/iot-tta#Smart_Product> ;
  rdfs:comment "iBeacon from Apple and Eddystone from Google are portable electronic devices that use network protocols such as NFC, RFID, optical tags, or BLE as hardware transmitters."@en .

<https://w3id.org/iot-tta#Edge_application>
  a owl:Class ;
  rdfs:subClassOf <https://w3id.org/iot-tta#Application> ;
  rdfs:comment "Applications based on edge computing - the term \"edge\" refers to any computational or network resource available between the data source and the cloud services."@en .

<https://w3id.org/iot-tta#Edge_security>
  a owl:Class ;
  rdfs:subClassOf <https://w3id.org/iot-tta#Edge_technology> ;
  rdfs:comment "The edge security must consider criteria based on memory size, computational cost, transmission speed, etc. Blockchain may offer security solutions."@en .

<https://w3id.org/iot-tta#Edge_technology>
  a owl:Class ;
  rdfs:subClassOf <https://w3id.org/iot-tta#Technology> ;
  rdfs:comment "The term edge refers to any computational or network resource available between the initial data source and the cloud services."@en .

<https://w3id.org/iot-tta#Electrical_Grids>
  a owl:Class ;
  rdfs:subClassOf <https://w3id.org/iot-tta#Purpose-built_Device> ;
  rdfs:comment "The administration of electrical grids once controlled by manual input and electrical relays have been replaced by industrial control systems (ICS)."@en .

<https://w3id.org/iot-tta#Ethics>
  a owl:Class ;
  rdfs:subClassOf <https://w3id.org/iot-tta#Capabilities> ;
  rdfs:comment "IoT systems should be ethics-compliant regarding the following key aspects: (a) human rights; (b) avoid subordination, manipulation, or stimulating addiction; (c) products and services aim to bring positive changes to the society, environment, persons, and economy."@en .

<https://w3id.org/iot-tta#Factory_Equipment>
  a owl:Class ;
  rdfs:subClassOf <https://w3id.org/iot-tta#Purpose-built_Device> ;
  rdfs:comment "The administration of factory equipment is performed by the industrial control systems (ICS)."@en .

<https://w3id.org/iot-tta#Factory_Floor>
  a owl:Class ;
  rdfs:subClassOf <https://w3id.org/iot-tta#Purpose-built_Device> ;
  rdfs:comment "The administration of factory floors is performed by the industrial control systems (ICS)."@en .

<https://w3id.org/iot-tta#Firmware>
  a owl:Class ;
  rdfs:subClassOf <https://w3id.org/iot-tta#Algorithm> ;
  rdfs:comment "In a Particle Photon application, a firmware program reads the value D0 of a pin, call the function Particle.publish() with one of the value “0” or “1” that is sent to the Particle cloud."@en .

<https://w3id.org/iot-tta#Flow>
  a owl:Class ;
  rdfs:subClassOf <https://w3id.org/iot-tta#Particle_Photon> ;
  rdfs:comment "Flow describes the Flow-Service-Quality semantics for a Particle Photon application that includes a Thingspeak subscriber, a WebHook, and a firmware program."@en .

<https://w3id.org/iot-tta#Gas_Meter>
  a owl:Class ;
  rdfs:subClassOf <https://w3id.org/iot-tta#Purpose-built_Device> ;
  rdfs:comment "The administration of gas meters is performed by the industrial control systems (ICS)"@en .

<https://w3id.org/iot-tta#Gateway>
  a owl:Class ;
  rdfs:subClassOf <https://w3id.org/iot-tta#Device> ;
  rdfs:comment "Gateways process the data from multiple devices and send them to the cloud"@en .

<https://w3id.org/iot-tta#Grid>
  a owl:Class ;
  rdfs:subClassOf <https://w3id.org/iot-tta#Support> ;
  rdfs:comment "Grid computing is a form of distributed computing based on independent computers connected to a network by a network interface, such as Ethernet."@en .

<https://w3id.org/iot-tta#HAT>
  a owl:Class ;
  rdfs:subClassOf <https://w3id.org/iot-tta#Sensor_Actuator> ;
  rdfs:comment "Modules that connect processing boards to computers and other objects"@en .

<https://w3id.org/iot-tta#HBase>
  a owl:Class ;
  rdfs:subClassOf <https://w3id.org/iot-tta#Tool> ;
  rdfs:comment "HBase is a non-relational distributed database developed as part of Apache Hadoop. HBase runs on top of the Hadoop Distributed File System, providing capabilities like Bigtable."@en .

<https://w3id.org/iot-tta#HTTP>
  a owl:Class ;
  rdfs:subClassOf <https://w3id.org/iot-tta#Protocol> ;
  rdfs:comment "HTTP (Hypertext Transfer Protocol) is part of the Internet protocol suite, allows access to pages from Web servers. HTTP is an application layer protocol according to the OSI reference model."@en .

<https://w3id.org/iot-tta#Hardware_Platform>
  a owl:Class ;
  rdfs:subClassOf <https://w3id.org/iot-tta#Digital> ;
  rdfs:comment "Examples of hardware platforms: a) microcontroller and computer platforms; b) HATs and Shields, modules that connect processing boards to computers and other objects."@en .

<https://w3id.org/iot-tta#Home_automation>
  a owl:Class ;
  rdfs:subClassOf <https://w3id.org/iot-tta#Smart_Product> ;
  rdfs:comment "smart IoT systems for home - smart lighting, intelligent heating and cooling, motorized blinds, and automated windows and doors, etc."@en .

<https://w3id.org/iot-tta#Hortonworks>
  a owl:Class ;
  rdfs:subClassOf <https://w3id.org/iot-tta#Tool> ;
  rdfs:comment "Hortonworks Data Platform (HDP) is a secure framework for distributed storage, processing of large, multi-source data sets, and data analysis."@en .

<https://w3id.org/iot-tta#Hub>
  a owl:Class ;
  rdfs:subClassOf <https://w3id.org/iot-tta#Control_engineering> ;
  rdfs:comment "The hub is a multi-port device that resends any received data packet to all of its ports except the one from which it received it."@en .

<https://w3id.org/iot-tta#ICS>
  a owl:Class ;
  rdfs:subClassOf <https://w3id.org/iot-tta#Industrial> ;
  rdfs:comment "ICS (industrial control systems)"@en .

<https://w3id.org/iot-tta#IP>
  a owl:Class ;
  rdfs:subClassOf <https://w3id.org/iot-tta#Protocol> ;
  rdfs:comment "IP (Internet Protocol) is a protocol for transmitting data over the Internet. The data is retrieved and divided into datagrams (IP packets) by the transport layer, transmitted over the Internet, and then reassembled by the network layer."@en .

<https://w3id.org/iot-tta#ISO_stack>
  a owl:Class ;
  rdfs:subClassOf <https://w3id.org/iot-tta#Protocol> ;
  rdfs:comment "ISO stack - protocols stack developed by the International Organization of Standardization (ISO) that works from the hardware physical layer to the software application layer."@en .

<https://w3id.org/iot-tta#IaaS>
  a owl:Class ;
  rdfs:subClassOf <https://w3id.org/iot-tta#Cloud_service> ;
  rdfs:comment "IaaS (Infrastructure-as-a-Service) is a cloud service for sharing distributed virtualized resources. The cloud provider owns and operates the hardware and software components and the data center."@en .

<https://w3id.org/iot-tta#Industrial>
  a owl:Class ;
  rdfs:subClassOf <https://w3id.org/iot-tta#Control_System> ;
  rdfs:comment "Examples of industrial control systems (ICS): manufacturing processes, power grids, oil and gas pipelines, etc."@en .

<https://w3id.org/iot-tta#Industrial_oven>
  a owl:Class ;
  rdfs:subClassOf <https://w3id.org/iot-tta#Industrial> ;
  rdfs:comment "Industrial ovens for a production line incorporate temperature sensors."@en .

<https://w3id.org/iot-tta#Internet_standard>
  a owl:Class ;
  rdfs:subClassOf <https://w3id.org/iot-tta#Logic> ;
  rdfs:comment "Internet standards and tools"@en .

<https://w3id.org/iot-tta#IoTLayers>
  a owl:Class ;
  rdfs:comment "IoT-TTA is a semantic ontology for the Internet of Things technologies, tools, and applications. IoT-TTA consists of a hierarchy of classes corresponding to the layers of a general IoT architecture: Device, Network, Support, Application, and Capabilities."@en .

<https://w3id.org/iot-tta#JSON_Web_Token>
  a owl:Class ;
  rdfs:subClassOf <https://w3id.org/iot-tta#Internet_standard> ;
  rdfs:comment "JSON Web Token is an Internet standard for creating data with optional signature and encryption."@en .

<https://w3id.org/iot-tta#Java>
  a owl:Class ;
  rdfs:subClassOf <https://w3id.org/iot-tta#Programming_Language> ;
  rdfs:comment "Java Programming for IoT Applications (e. g. IoT Java Application with Eclipse Kura)"@en .

<https://w3id.org/iot-tta#Kafka>
  a owl:Class ;
  rdfs:subClassOf <https://w3id.org/iot-tta#Distributed_system> ;
  rdfs:comment "Kafka is a distributed log messaging system. Apache Kafka is a distributed event streaming platform used for data pipelines, data integration, and streaming analytics."@en ;
  rdfs:label "Kafka"@en .

<https://w3id.org/iot-tta#LoRa>
  a owl:Class ;
  rdfs:subClassOf <https://w3id.org/iot-tta#Sensor_Actuator> ;
  rdfs:comment "LoRa (Long Range) performs the transmission with low power consumption, using the radio communication technique. LoRa devices have geolocation capabilities."@en .

<https://w3id.org/iot-tta#LoRaWan>
  a owl:Class ;
  rdfs:subClassOf <https://w3id.org/iot-tta#Sensor_Actuator> ;
  rdfs:comment "LoRaWAN (protocol above LoRa) - LoRaWAN is a cloud-based Medium Access Control (MAC) layer protocol for managing communication between gateways and end-node devices."@en .

<https://w3id.org/iot-tta#LoWPAN>
  a owl:Class ;
  rdfs:subClassOf <https://w3id.org/iot-tta#Protocol> ;
  rdfs:comment "The LoWPAN protocol belongs to the Internet layer and is extended from IP. It works on Low Power and Wireless Personal Area Network i.e., LoWPAN, and comprises an edge router and sensor nodes."@en .

<https://w3id.org/iot-tta#Logic>
  a owl:Class ;
  rdfs:subClassOf <https://w3id.org/iot-tta#Digital> ;
  owl:disjointWith <https://w3id.org/iot-tta#Smart_Product> ;
  rdfs:comment "Logic class contains algorithms, Web technologies, tools, programming languages, and Internet protocols."@en .

<https://w3id.org/iot-tta#MQTT>
  a owl:Class ;
  rdfs:subClassOf <https://w3id.org/iot-tta#Protocol> ;
  rdfs:comment "MQTT (Message Queue Telemetry Transport) is a standard IoT protocol that transfers data provided by sensors and performs communications via satellite."@en .

<https://w3id.org/iot-tta#MQTT_streams>
  a owl:Class ;
  rdfs:subClassOf <https://w3id.org/iot-tta#Data> ;
  rdfs:comment "MQTT (Message Queue Telemetry Transport) is a data streaming standard based on publish-subscribe networks that can transport messages from devices to a server. Clients connect to a central server and publish certain data. Cloud services can automatically show MQTT streams."@en .

<https://w3id.org/iot-tta#Machine_Learning>
  a owl:Class ;
  rdfs:subClassOf <https://w3id.org/iot-tta#Algorithm> ;
  rdfs:comment "The cloud ensures an efficient and scalable architecture for computation, data storage, and machine learning. Tools for machine learning: Mahout, Spark ML, TensorFlow, and Mllib."@en .

<https://w3id.org/iot-tta#Machine_learning>
  a owl:Class ;
  rdfs:subClassOf <https://w3id.org/iot-tta#Application> ;
  rdfs:comment "Machine learning applications including artificial neural networks, data mining, genetic algorithms. Tools for machine learning: Mahout, Spark ML, Mllib, Tensor Flow, Theano, Python, Weka, R, Octave, etc."@en .

<https://w3id.org/iot-tta#Mahout>
  a owl:Class ;
  rdfs:subClassOf <https://w3id.org/iot-tta#Machine_Learning> ;
  rdfs:comment "Apache Mahout provides distributed machine learning algorithms. The Apache platforms use Hadoop or Spark. Mahout includes Java and Scala libraries and collections."@en .

<https://w3id.org/iot-tta#Management>
  a owl:Class ;
  rdfs:subClassOf <https://w3id.org/iot-tta#Capabilities> ;
  rdfs:comment "Device and data management - Device management covers three operations: adding new devices, monitoring, and updating devices. The high-performance access to data from IoT applications can be maintained using Cloud Storage, an online storage service."@en .

<https://w3id.org/iot-tta#MapR>
  a owl:Class ;
  rdfs:subClassOf <https://w3id.org/iot-tta#Tool> ;
  rdfs:comment "MapReduce is a programming model for processing big data sets with a parallel, distributed algorithm on a cluster of computers. A MapReduce system has usually three operations: map, shuffle, and reduce. A popular open-source implementation is part of Apache Hadoop."@en .

<https://w3id.org/iot-tta#Mesos>
  a owl:Class ;
  rdfs:subClassOf <https://w3id.org/iot-tta#Distributed_operating_system> ;
  rdfs:comment "Mesos is a distributed operating system that runs on every machine. The Mesos kernel provides applications like Hadoop, Spark, Kafka and ensures resource management and scheduling in cloud environment."@en .

<https://w3id.org/iot-tta#Microcontroller>
  a owl:Class ;
  rdfs:subClassOf <https://w3id.org/iot-tta#Hardware_Platform> ;
  rdfs:comment "CPU on a single chip; RAM, ROM, EEPROM, Timer, I/O, Serial Interface"@en .

<https://w3id.org/iot-tta#Microprocessor>
  a owl:Class ;
  rdfs:subClassOf <https://w3id.org/iot-tta#Hardware_Platform> ;
  rdfs:comment "CPU and several supporting chips; RAM, ROM, Input, Output, Serial Interface, Timers"@en .

<https://w3id.org/iot-tta#Microprocessor_Platform>
  a owl:Class ;
  rdfs:subClassOf <https://w3id.org/iot-tta#Gateway> ;
  owl:disjointWith <https://w3id.org/iot-tta#Smartphone> ;
  rdfs:comment "Gateway devices (e.g. microprocessor platforms) enable a secure connection to the cloud and can do real-time analytics or machine learning"@en .

<https://w3id.org/iot-tta#Mllib>
  a owl:Class ;
  rdfs:subClassOf <https://w3id.org/iot-tta#Machine_Learning> ;
  rdfs:comment "MLlib (Machine Learning Library for Spark) contains algorithms such as classification, regression, clustering, and collaborative filtering."@en .

<https://w3id.org/iot-tta#Mobile_node>
  a owl:Class ;
  rdfs:subClassOf <https://w3id.org/iot-tta#Wireless_sensor_network> ;
  rdfs:comment "In a wireless sensor network, a mobile node identifies nearby network nodes and logins with a password using the SAMPL protocol, gateway, and Publish-Subscribe service."@en .

<https://w3id.org/iot-tta#NFC_tag>
  a owl:Class ;
  rdfs:subClassOf <https://w3id.org/iot-tta#Protocol> ;
  rdfs:comment "NFC tags (Near Field Communication limited to high-frequency) are protocols that identify passive things. NFC tags are passive, meaning they don't have any power source. They take power from the device that reads them, through magnetic induction."@en .

<https://w3id.org/iot-tta#Network>
  a owl:Class ;
  rdfs:subClassOf <https://w3id.org/iot-tta#IoTLayers> ;
  rdfs:comment "\"Network\" represents a layer of the IoT architecture. The networking layer concerns data transmission among devices, the types of communications, and some network protocols used in IoT."@en .

<https://w3id.org/iot-tta#Network_card>
  a owl:Class ;
  rdfs:subClassOf <https://w3id.org/iot-tta#Computer_architecture> ;
  rdfs:comment "The network card, also called \"network adapter\" or \"network interface card\", is a circuit that allows communication between the computer and the network (Internet, LAN)."@en .

<https://w3id.org/iot-tta#NoSQL_Data>
  a owl:Class ;
  rdfs:subClassOf <https://w3id.org/iot-tta#Data> ;
  rdfs:comment "NoSQL database is a non-relational database. Types of NoSQL databases: document databases, key-value databases, wide-column stores, and graph databases. Ex. Azure Cosmos DB, Oracle NoSQL, MongoDB, Azure Cosmos DB, HBase databases, applications that use Hadoop, etc."@en .

<https://w3id.org/iot-tta#Node>
  a owl:Class ;
  rdfs:subClassOf <https://w3id.org/iot-tta#Web_Technology> ;
  rdfs:comment "Software platforms (e.g., Python, Django, Node) and Web technologies are integrated with hardware components of the IoT systems. Node or NodeJS is a back-end Javascript runtime environment. Features: fast and real-time execution and good integration with IoT protocols."@en .

<https://w3id.org/iot-tta#Oil_Pipeline_Control>
  a owl:Class ;
  rdfs:subClassOf <https://w3id.org/iot-tta#Purpose-built_Device> ;
  rdfs:comment "Sensors are embedded into purpose-built devices such as oil pipeline control systems."@en .

<https://w3id.org/iot-tta#Optical_tag>
  a owl:Class ;
  rdfs:subClassOf <https://w3id.org/iot-tta#Protocol> ;
  rdfs:comment "Identifying passive things can be performed using protocols such as optical tags, as hardware transmitters to nearby portable electronic devices."@en .

<https://w3id.org/iot-tta#PAN>
  a owl:Class ;
  rdfs:subClassOf <https://w3id.org/iot-tta#Protocol> ;
  rdfs:comment "PAN (Personal Area Network) is a network protocol that ensures the connection between devices within a radius of 10 meters. A PAN usually involves a PC, phone, personal digital assistant, tablet, printer, speakers, video game consoles, etc."@en .

<https://w3id.org/iot-tta#PLC>
  a owl:Class ;
  rdfs:subClassOf <https://w3id.org/iot-tta#Hardware_Platform> ;
  rdfs:comment "PLC (Programmable Logic Controller) is a ruggedized computer. Features: valves, sensors, motors. PLC programming languages: Ladder Logic, Function Block Diagram, Sequential Function Chart; Connection with SCADA"@en .

<https://w3id.org/iot-tta#PaaS>
  a owl:Class ;
  rdfs:subClassOf <https://w3id.org/iot-tta#Cloud_service> ;
  rdfs:comment "PaaS (Platform-as-a-Service) is a cloud service that provides a virtual environment. PaaS provides the infrastructure and middleware components for developing and managing mobile and web applications in the cloud."@en .

<https://w3id.org/iot-tta#Particle_Photon>
  a owl:Class ;
  rdfs:subClassOf <https://w3id.org/iot-tta#Microcontroller> ;
  rdfs:comment "A Particle Photon application used for highlighting the Flow-Service-Quality semantics"@en .

<https://w3id.org/iot-tta#Particle_cloud>
  a owl:Class ;
  rdfs:subClassOf <https://w3id.org/iot-tta#Particle_Photon> ;
  rdfs:comment "Particle cloud describes the Flow-Service-Quality semantics for a Particle Photon application using the properties \"wire\", \"read\", \"send\", \"request\" and constraints based on \"hasTimeLimit\" and \"hasValueConnection\"."@en .

<https://w3id.org/iot-tta#Passive_things>
  a owl:Class ;
  rdfs:subClassOf <https://w3id.org/iot-tta#Smart_Product> ;
  rdfs:comment "“Passive things” have sensors that do not require external power, they just react to inputs from their environment."@en .

<https://w3id.org/iot-tta#Peer-to-peer_system>
  a owl:Class ;
  rdfs:subClassOf <https://w3id.org/iot-tta#Support> ;
  rdfs:comment "A peer-to-peer system is a computer network that enables the sharing of network resources, computational power, and data storage, in an equal way between peers."@en .

<https://w3id.org/iot-tta#Privacy>
  a owl:Class ;
  rdfs:subClassOf <https://w3id.org/iot-tta#Capabilities> ;
  rdfs:comment "Privacy and data protection throughout their use and processing personal data"@en .

<https://w3id.org/iot-tta#Processing_Board>
  a owl:Class ;
  rdfs:subClassOf <https://w3id.org/iot-tta#Sensor_Actuator> ;
  rdfs:comment "The processing board is an IoT board with a processor, memory (MicroSD, RAM), low-level IO, multimedia, inputs, connectivity, and power (usually USB connectors, headers, etc)."@en .

<https://w3id.org/iot-tta#Programming_Language>
  a owl:Class ;
  rdfs:subClassOf <https://w3id.org/iot-tta#Logic> ;
  rdfs:comment "IoT devices use certain programming languages to process and control data transfer (e.g. Raspberry Pi, Programmable Logic Controller, C, Java, Python)."@en .

<https://w3id.org/iot-tta#Protocol>
  a owl:Class ;
  rdfs:subClassOf <https://w3id.org/iot-tta#Network> ;
  rdfs:comment "A network protocol is a communication protocol implemented on a computer network or telecommunications network. Network protocols form protocol layers corresponding to OSI levels."@en .

<https://w3id.org/iot-tta#Purpose-built_Device>
  a owl:Class ;
  rdfs:subClassOf <https://w3id.org/iot-tta#Digital> ;
  rdfs:comment "Sensors are usually incorporated into connected objects or purpose-built devices such as components of a city’s infrastructure, controllers for factory equipment, oil pipeline control, etc."@en .

<https://w3id.org/iot-tta#Python>
  a owl:Class ;
  rdfs:subClassOf <https://w3id.org/iot-tta#Programming_Language> ;
  rdfs:comment "Python programming for IoT systems uses libraries/packages such as numpy,  request, paho.mqtt.client, Countly, matplotlib, etc."@en .

<https://w3id.org/iot-tta#RFID_tag>
  a owl:Class ;
  rdfs:subClassOf <https://w3id.org/iot-tta#Protocol> ;
  rdfs:comment "RFID tags (Radio Frequency Identification) are used as hardware transmitters to nearby portable electronic devices, for identifying passive things."@en .

<https://w3id.org/iot-tta#RTD_sensor>
  a owl:Class ;
  rdfs:subClassOf <https://w3id.org/iot-tta#Sensor_Actuator> ;
  rdfs:comment "RTD sensors of an industrial oven."@en .

<https://w3id.org/iot-tta#Raspberry_Pi>
  a owl:Class ;
  rdfs:subClassOf <https://w3id.org/iot-tta#Microcontroller> ;
  rdfs:comment "Raspberry Pi uses operating systems such as Raspberry Pi OS, Raspbian, some versions of Linux, or Windows 10 IoT Core. Tools and programming languages: GPIO (general-purpose input/output) pins; PWM - Pulse-Width Modulation, Python, C/C++, Wyliodrin Studio"@en .

<https://w3id.org/iot-tta#Raspberyy_Pi_4B>
  a owl:Class ;
  rdfs:subClassOf <https://w3id.org/iot-tta#Raspberry_Pi> ;
  rdfs:comment "Raspberry Pi uses operating systems like Linux, Raspbian (a Debian GNU/Linux), Raspberry Pi OS Lite, etc. Features: GPIO (general-purpose input/output) pins, PWM - Pulse-Width Modulation, programming languages and tools: GPIO with Scratch, Python, C/C++, Processing, Wyliodrin Studio, etc."@en .

<https://w3id.org/iot-tta#Router>
  a owl:Class ;
  rdfs:subClassOf <https://w3id.org/iot-tta#Control_engineering> ;
  rdfs:comment "A router connects two or more computer networks using packet switching. These networks can be wired or wireless. A wireless router exchanges information between the network and the Internet using radio signals."@en .

<https://w3id.org/iot-tta#SAMPL>
  a owl:Class ;
  rdfs:subClassOf <https://w3id.org/iot-tta#Protocol> ;
  rdfs:comment "SAMPL is a compact network layer that operates on top of a low-power CSMA/CA-based MAC protocol. SAMPL operates as part of the sensor Andrew project at Carnegie Mellon University and FireFly wireless sensor networks."@en .

<https://w3id.org/iot-tta#SCADA>
  a owl:Class ;
  rdfs:subClassOf <https://w3id.org/iot-tta#Hardware_Platform> ;
  rdfs:comment "SCADA (Supervisory Control and Data Acquisition) is a control system comprising sensors, PLC (Programmable Logic Controllers), networked data communications, GUI for supervision of processes, and computers."@en .

<https://w3id.org/iot-tta#SCADA_capability>
  a owl:Class ;
  rdfs:subClassOf <https://w3id.org/iot-tta#SCADA> ;
  rdfs:comment "SCADA is used to centrally manage and monitor the various complex systems in an industrial setting. SCADA and ICS sensors make up the complex distributed industrial computing architecture."@en .

<https://w3id.org/iot-tta#SCADA_common_protocol>
  a owl:Class ;
  rdfs:subClassOf <https://w3id.org/iot-tta#SCADA> ;
  rdfs:comment "The common protocols on which SCADA systems operate and transfer data are Modbus and BACnet."@en .

<https://w3id.org/iot-tta#SCADA_demand>
  a owl:Class ;
  rdfs:subClassOf <https://w3id.org/iot-tta#SCADA> ;
  rdfs:comment "For SCADA systems, the demand for remote management and monitoring increased."@en .

<https://w3id.org/iot-tta#SCADA_problem>
  a owl:Class ;
  rdfs:subClassOf <https://w3id.org/iot-tta#SCADA> ;
  rdfs:comment "The SCADA common protocols such as Modbus and BACnet lack the built-in security measures required to adequately defend against new threats directed at critical infrastructure."@en .

<https://w3id.org/iot-tta#SCADA_solution>
  a owl:Class ;
  rdfs:subClassOf <https://w3id.org/iot-tta#SCADA> ;
  rdfs:comment "Insecure SCADA protocols were layered into Ethernet and TCP/IP to support long-distance communication."@en .

<https://w3id.org/iot-tta#SCADA_today_protocol>
  a owl:Class ;
  rdfs:subClassOf <https://w3id.org/iot-tta#SCADA> ;
  rdfs:comment "Ethernet and TCP/IP protocols are still used today by SCADA around the world."@en .

<https://w3id.org/iot-tta#SOA>
  a owl:Class ;
  rdfs:subClassOf <https://w3id.org/iot-tta#Application> ;
  rdfs:comment "Applications based on the Service-Oriented Architecture (SOA)"@en .

<https://w3id.org/iot-tta#SaaS>
  a owl:Class ;
  rdfs:subClassOf <https://w3id.org/iot-tta#Cloud_service> ;
  rdfs:comment "SaaS (Software-as-a-Service) is a cloud service that supports running end-user applications. The cloud service provider develops and maintains software for cloud applications and makes the software available to its customers over the Internet."@en .

<https://w3id.org/iot-tta#Satellite>
  a owl:Class ;
  rdfs:subClassOf <https://w3id.org/iot-tta#Hardware_Platform> ;
  rdfs:comment "MQTT performs communications via satellite"@en .

<https://w3id.org/iot-tta#Security>
  a owl:Class ;
  rdfs:subClassOf <https://w3id.org/iot-tta#Capabilities> ;
  rdfs:comment "The security concerns for the IoT systems refer to denial-of-service (DoS) attacks through concurrent requests, weak protection credentials, insecure communication between devices, recovery, data backup during a system interruption, limited network visibility, etc."@en .

<https://w3id.org/iot-tta#Sensor_Actuator>
  a owl:Class ;
  rdfs:subClassOf <https://w3id.org/iot-tta#Device> ;
  rdfs:comment "The modules with sensors or actuators connect processing boards to computers and other devices. Unlike simple sensors, actuators can make changes in the environment."@en .

<https://w3id.org/iot-tta#Shield>
  a owl:Class ;
  rdfs:subClassOf <https://w3id.org/iot-tta#Sensor_Actuator> ;
  rdfs:comment "Modules that connect processing boards to computers and other objects"@en .

<https://w3id.org/iot-tta#Smart_Product>
  a owl:Class ;
  rdfs:subClassOf <https://w3id.org/iot-tta#Digital> ;
  rdfs:comment "Smart products are controlled and managed using Web technologies and software platforms."@en .

<https://w3id.org/iot-tta#Smartphone>
  a owl:Class ;
  rdfs:subClassOf <https://w3id.org/iot-tta#Gateway> ;
  rdfs:comment "Smartphones are gateway devices that enable data connectivity through their set of sensors: GPS, biometrics, Bluetooth, heart rate monitor, ECG, barcode readers, etc."@en .

<https://w3id.org/iot-tta#Spark>
  a owl:Class ;
  rdfs:subClassOf <https://w3id.org/iot-tta#Machine_Learning>, <https://w3id.org/iot-tta#Tool> ;
  rdfs:comment "Apache Spark is part of the Hadoop system. Spark allows big data processing and building machine learning models such as regression, classification, clustering, and recommendation systems in a distributed processing environment."@en .

<https://w3id.org/iot-tta#Subscriber>
  a owl:Class ;
  rdfs:subClassOf <https://w3id.org/iot-tta#Tool> ;
  rdfs:comment "A subscriber requests information about a specific topic in a publish/subscribe network and receives messages from more publishers. A subscription is a request sent by the subscriber to receive messages on a particular topic."@en .

<https://w3id.org/iot-tta#Support>
  a owl:Class ;
  rdfs:subClassOf <https://w3id.org/iot-tta#IoTLayers> ;
  rdfs:comment "\"Support\" represents a layer of the IoT architecture. The support layer is represented by distributed systems (cloud systems)."@en .

<https://w3id.org/iot-tta#Switch>
  a owl:Class ;
  rdfs:subClassOf <https://w3id.org/iot-tta#Computer_architecture> ;
  rdfs:comment "In a computer network, a switch interconnects different network segments based on Media Access Control (MAC) addresses. A MAC address is a 6-byte integer on Token-ring or Ethernet networks used to identify a computer on a local network."@en .

<https://w3id.org/iot-tta#TCP>
  a owl:Class ;
  rdfs:subClassOf <https://w3id.org/iot-tta#Protocol> ;
  rdfs:comment "TCP (Transmission Control Protocol) corresponds to the Transport layer of the Internet protocol suite TCP/IP. Common applications using TCP are the World Wide Web (WWW), e-mail, and file transfer (FTP)."@en .

<https://w3id.org/iot-tta#Technology>
  a owl:Class ;
  rdfs:subClassOf <https://w3id.org/iot-tta#Support> ;
  rdfs:comment "Technologies used for distributed systems: Blockchain, big data processing, edge technology, computer cluster, data analysis, deep learning, etc."@en .

<https://w3id.org/iot-tta#Tool>
  a owl:Class ;
  rdfs:subClassOf <https://w3id.org/iot-tta#Support> ;
  rdfs:comment "Tools for distributed computing technologies like MapReduce, Cloudera, Spark, HBase, Hortonworks, Subscriber, Watson IoT, etc."@en .

<https://w3id.org/iot-tta#Transducer>
  a owl:Class ;
  rdfs:subClassOf <https://w3id.org/iot-tta#Sensor_Actuator> ;
  rdfs:comment "A transducer converts a signal from one physical structure to another and converts one type of energy into another type. There are two types of transducers: sensors and actuators. Sensors are used for sensing things and devices etc."@en .

<https://w3id.org/iot-tta#UDP>
  a owl:Class ;
  rdfs:subClassOf <https://w3id.org/iot-tta#Protocol> ;
  rdfs:comment "UDP (User Datagram Protocol) corresponds to the Transport layer of the Internet protocol suite TCP/IP. UDP ensures the delivery of messages over a network, but unlike the TCP protocol, information packets are generally sent without receipt confirmation."@en .

<https://w3id.org/iot-tta#WPAN>
  a owl:Class ;
  rdfs:subClassOf <https://w3id.org/iot-tta#Protocol> ;
  rdfs:comment "WPAN (Wireless Personal Area Network) is a PAN that ensures the connection between devices through wireless, within a radius of 10 meters. WPAN includes wearable devices, USB flash drives, wireless mouse, Bluetooth, Wi-Fi, thermostats, security systems, lighting controls, motion sensors, etc."@en .

<https://w3id.org/iot-tta#Watson_IoT>
  a owl:Class ;
  rdfs:subClassOf <https://w3id.org/iot-tta#Tool> ;
  rdfs:comment "IBM Watson IoT Platform manages connected devices and offers access to live and historical data for IoT applications."@en .

<https://w3id.org/iot-tta#Web_Technology>
  a owl:Class ;
  rdfs:subClassOf <https://w3id.org/iot-tta#Logic> ;
  rdfs:comment "Hardware components of an IoT system are integrated with certain Web technologies and software platforms."@en .

<https://w3id.org/iot-tta#Web_socket>
  a owl:Class ;
  rdfs:subClassOf <https://w3id.org/iot-tta#Application> ;
  rdfs:comment "Applications that use the WebSocket API"@en .

<https://w3id.org/iot-tta#Wireless_sensor_network>
  a owl:Class ;
  rdfs:subClassOf <https://w3id.org/iot-tta#Sensor_Actuator> ;
  rdfs:comment "Wireless Sensor Networks - Sensor nodes are used with an onboard processor that manages and monitors the environment in a certain area. They are connected to the base station through the Internet to share data."@en .

<https://w3id.org/iot-tta#XML>
  a owl:Class ;
  rdfs:subClassOf <https://w3id.org/iot-tta#Internet_standard> ;
  rdfs:comment "XML (Extensible Markup Language) is a markup language recommended by the W3C (World Wide Web Consortium) and used for storing unstructured and semi-structured data and transferring data between Internet applications."@en .

<https://w3id.org/iot-tta#XMPP>
  a owl:Class ;
  rdfs:subClassOf <https://w3id.org/iot-tta#Protocol> ;
  rdfs:comment "XMPP (Extensible Messaging and Presence Protocol) is an open standard that offers support for middleware applications, invisible messaging with the TCP network layer (hides the details of messaging), voice and video calls, collaboration, and generalized routing of XML data."@en .

<https://w3id.org/iot-tta#YARN>
  a owl:Class ;
  rdfs:subClassOf <https://w3id.org/iot-tta#Distributed_operating_system> ;
  rdfs:comment "Yarn (Yet Another Resource Negotiator) is a distributed operating system. YARN allows the resource management and scheduling jobs in Hadoop."@en .

<https://w3id.org/iot-tta#health-monitoring_system>
  a owl:Class ;
  rdfs:subClassOf <https://w3id.org/iot-tta#Smart_Product> ;
  rdfs:comment "Remote patient monitoring devices: glucometer, pulse oximeter, thermometer, ECG, digital stethoscope, wearables, scales, etc."@en .

<https://w3id.org/iot-tta#iBeacon>
  a owl:Class ;
  rdfs:subClassOf <https://w3id.org/iot-tta#Smart_Product> ;
  rdfs:comment "iBeacon from Apple and Eddystone from Google are portable electronic devices that use network protocols such as NFC, RFID, optical tags, or BLE as hardware transmitters."@en .

<https://w3id.org/iot-tta#Distributed_authentication>
  a owl:NamedIndividual, <https://w3id.org/iot-tta#Blockchain_solution> ;
  rdfs:comment "Distributed_authentication (Individual): a Blockchain solution"@en .

<https://w3id.org/iot-tta#Access_control>
  a owl:NamedIndividual, <https://w3id.org/iot-tta#Blockchain_solution> ;
  rdfs:comment "Access_control (Individual): a Blockchain solution"@en .

<https://w3id.org/iot-tta#Apache_Hadoop>
  a owl:NamedIndividual, <https://w3id.org/iot-tta#Tool> ;
  ns0:isToolFor ns0:Large_data_stream ;
  rdfs:comment "Apache_Hadoop (Individual): a Tool with Object property assertions (isToolFor)"@en .

ns0:Apache_IoT_edge
  a owl:NamedIndividual, ns0:Tool ;
  rdfs:comment "Apache_IoT_edge (Individual): a Tool"@en .

ns0:Autonomous_vehicle
  a owl:NamedIndividual, ns0:Edge_application ;
  ns0:hasTechnology ns0:Micro_data_center ;
  rdfs:comment "Autonomous_vehicle (Individual): an Edge application with Object property assertions (hasTechnology)"@en .

ns0:Avoid_synchronization
  a owl:NamedIndividual, ns0:Cloud_service ;
  rdfs:comment "Avoid_synchronization (Individual): a Cloud service"@en .

ns0:Azure_IoT_edge
  a owl:NamedIndividual, ns0:Tool ;
  rdfs:comment "Azure_IoT_edge (Individual): a Tool"@en .

ns0:BACnet
  a owl:NamedIndividual, ns0:SCADA_common_protocol ;
  ns0:Lack_security_measure ns0:Threats_at_critical_infrastructure ;
  ns0:Protocols_were_layered ns0:Ethernet ;
  rdfs:comment "BACnet (Individual): a SCADA common protocol with Object property assertions (Protocols_were_layered, Lack_security_measure)"@en .

ns0:Blockchain_algorithm
  a owl:NamedIndividual, ns0:Blockchain ;
  ns0:hasProblem ns0:Energy_managed ;
  rdfs:comment "Blockchain_algorithm (Individual): of Blockchain type with Object property assertions (hasProblem)"@en .

ns0:Centralized_service
  a owl:NamedIndividual, ns0:Cloud_service ;
  rdfs:comment "Centralized_service (Individual): a Cloud service"@en .

ns0:Cloud_Photon1
  a owl:NamedIndividual, ns0:Particle_cloud ;
  ns0:request ns0:Thingspeak1 ;
  rdfs:comment "Cloud_Photon1 (Individual): a Particle_cloud with Object property assertions (request)"@en .

ns0:Cloud_Photon2
  a owl:NamedIndividual, ns0:Particle_cloud ;
  ns0:request ns0:Thingspeak2 ;
  rdfs:comment "Cloud_Photon2 (Individual): a Particle_cloud with Object property assertions (request)"@en .

ns0:Cloud_gaming
  a owl:NamedIndividual, ns0:Edge_application ;
  ns0:hasTechnology ns0:Micro_data_center ;
  rdfs:comment "Cloud_gaming (Individual): an Edge application with Object property assertions (hasTechnology)"@en .

ns0:Cluster1
  a owl:NamedIndividual, ns0:Computer_cluster ;
  rdfs:comment "Cluster1 (Individual): a Computer cluster"@en .

ns0:Cluster2
  a owl:NamedIndividual, ns0:Computer_cluster ;
  rdfs:comment "Cluster2 (Individual): a Computer cluster"@en .

ns0:Computational_cost
  a owl:NamedIndividual, ns0:Edge_security ;
  ns0:best_Practices ns0:Smart_grid ;
  ns0:has_SecuritySolution ns0:Correct_Edge_implementation ;
  rdfs:comment "Computational_cost (Individual): of Edge security type with Object property assertions (has_SecuritySolution, best_Practices)"@en .

ns0:Connection1
  a owl:NamedIndividual, ns0:Flow ;
  ns0:read ns0:Particle_publish1 ;
  ns0:hasValueConnection 1 ;
  rdfs:comment "Connection1 (Individual): a Flow with Object property assertions (read), Data property assertions (hasValueConnection)"@en .

ns0:Connection2
  a owl:NamedIndividual, ns0:Flow ;
  ns0:read ns0:Particle_publish2 ;
  ns0:hasValueConnection 0 ;
  rdfs:comment "Connection2 (Individual): a Flow with Object property assertions (read), Data property assertions (hasValueConnection)"@en .

ns0:Correct_Edge_implementation
  a owl:NamedIndividual, ns0:Blockchain_solution ;
  rdfs:comment "Correct_Edge_implementation (Individual): a Blockchain solution"@en .

ns0:DC1
  a owl:NamedIndividual, ns0:Data_center ;
  ns0:hasService ns0:Centralized_service ;
  ns0:useAlgorithm ns0:Paxos ;
  rdfs:comment "DC1 (Individual): a Data center with Object property assertions (hasService, useAlgorithm)"@en .

ns0:DC2
  a owl:NamedIndividual, ns0:Data_center ;
  ns0:hasService ns0:Avoid_synchronization ;
  ns0:useAlgorithm ns0:Zookeeper ;
  rdfs:comment "DC2 (Individual): a Data center with Object property assertions (hasService, useAlgorithm)"@en .

ns0:DC3
  a owl:NamedIndividual, ns0:Data_center ;
  ns0:hasService ns0:Avoid_synchronization ;
  ns0:useAlgorithm ns0:Paxos ;
  rdfs:comment "DC3 (Individual): a Data center with Object property assertions (hasService, useAlgorithm)"@en .

ns0:DC4
  a owl:NamedIndividual, ns0:Data_center ;
  ns0:useAlgorithm ns0:Paxos ;
  rdfs:comment "DC4 (Individual): a Data center with Object property assertions (useAlgorithm)"@en .

ns0:Data_protection
  a owl:NamedIndividual, ns0:Blockchain_solution ;
  rdfs:comment "Data_protection (Individual): a Blockchain solution with Object property assertions (hasSolution)"@en .

ns0:Data_security_risk
  a owl:NamedIndividual, ns0:SCADA_problem ;
  ns0:countermeasure ns0:End-to-end_encryption, ns0:Strong_authentication ;
  rdfs:comment "Data_security_risk (Individual): a SCADA problem with Object property assertions (countermeasure)"@en .

ns0:Data_stream_continue
  a owl:NamedIndividual, ns0:Blockchain ;
  ns0:hasProblem ns0:Throughput_limited ;
  rdfs:comment "Data_stream_continue (Individual): of Blockchain type with Object property assertions (hasProblem)"@en .

ns0:Deep_learning_algorithm
  a owl:NamedIndividual, ns0:Deep_learning ;
  rdfs:comment "Deep_learning_algorithm (Individual): of Deep learning type with Object property assertions (hasTool)"@en .

ns0:Distributed_capability
  a owl:NamedIndividual, ns0:BigData_capability ;
  rdfs:comment "Distributed_capability (Individual): Big data capability"@en .

ns0:End-to-end_encryption
  a owl:NamedIndividual, ns0:SCADA_solution ;
  rdfs:comment "End-to-end_encryption (Object property): a SCADA_solution"@en .

ns0:Energy_managed
  a owl:NamedIndividual, ns0:Blockchain_problem ;
  ns0:hasSolution ns0:Improve_central_algorithm ;
  rdfs:comment "Energy_managed (Individual): a Blockchain problem with Object property assertions (hasSolution)"@en .

ns0:Ethernet
  a owl:NamedIndividual, ns0:SCADA_today_protocol ;
  ns0:Support_communication ns0:Long-distance_communication ;
  rdfs:comment "Ethernet (Individual): a SCADA todat protocol with Object property assertions (Support_communication)"@en .

ns0:Hadoop
  a owl:NamedIndividual, ns0:Tool ;
  ns0:isUsedBy ns0:Cluster1, ns0:Cluster2 ;
  rdfs:comment "Hadoop (Individual): a Tool with Object property assertions (isUsedBy)"@en .

ns0:Improve_central_algorithm
  a owl:NamedIndividual, ns0:Blockchain_solution ;
  rdfs:comment "Improve_central_algorithm (Individual): a Blockchain solution"@en .

ns0:Integrity_assurance
  a owl:NamedIndividual, ns0:Blockchain_solution ;
  rdfs:comment "Integrity_assurance (Individual): a Blockchain solution"@en .

ns0:Large_data_stream
  a owl:NamedIndividual, ns0:BigData ;
  ns0:isProcessed ns0:Distributed_capability ;
  rdfs:comment "Large_data_stream (Individual): Big Data type with Object property assertions (isProcessed)"@en .

ns0:Long-distance_communication
  a owl:NamedIndividual, ns0:SCADA_capability ;
  rdfs:comment "Long-distance_communication (Individual): a SCADA_capability"@en .

ns0:Maintain_configuration
  a owl:NamedIndividual, ns0:Cloud_service ;
  rdfs:comment "Maintain_configuration (Individual): a Cloud service"@en .

ns0:MapReduce
  a owl:NamedIndividual, ns0:Tool ;
  ns0:isApplied ns0:Cluster1 ;
  rdfs:comment "MapReduce (Individual): a Tool with Object property assertions (isApplied)"@en .

ns0:Micro_data_center
  a owl:NamedIndividual, ns0:Edge_technology ;
  ns0:hasTool ns0:Azure_IoT_edge ;
  rdfs:comment "Micro_data_center (Individual): an edge technology with Object property assertions (hasTool)"@en .

ns0:Modbus
  a owl:NamedIndividual, ns0:SCADA_common_protocol ;
  ns0:Lack_security_measure ns0:Threats_at_critical_infrastructure ;
  ns0:Protocols_were_layered ns0:TCP_IP ;
  rdfs:comment "Modbus (Individual): a SCADA common protocol with Object property assertions (Lack_security_measure, Protocols_were_layered)"@en .

ns0:OPC_servers
  a owl:NamedIndividual, ns0:Edge_technology ;
  ns0:hasTool ns0:Apache_IoT_edge ;
  rdfs:comment "OPC_servers (Individual): an edge technology with Object property assertions (hasTool)"@en .

ns0:Oven1
  a owl:NamedIndividual, ns0:Industrial_oven ;
  ns0:hasTemperatureRange 5.080000e+2 ;
  rdfs:comment "Oven1 (Individual): an Industrial_oven with Data property assertions (hasTemperatureRange)"@en .

ns0:Oven2
  a owl:NamedIndividual, ns0:Industrial_oven ;
  ns0:hasTemperatureRange 5.020000e+2 ;
  rdfs:comment "Oven2 (Individual): an Industrial_oven with Data property assertions (hasTemperatureRange)"@en .

ns0:Oven3
  a owl:NamedIndividual, ns0:Industrial_oven ;
  ns0:hasTemperatureRange 5.010000e+2 ;
  rdfs:comment "Oven3 (Individual): an Industrial_oven with Data property assertions (hasTemperatureRange)"@en .

ns0:Oven4
  a owl:NamedIndividual, ns0:Industrial_oven ;
  ns0:hasTemperatureRange 5.060000e+2 ;
  rdfs:comment "Oven4 (Individual): an Industrial_oven with Data property assertions (hasTemperatureRange)"@en .

ns0:Oven5
  a owl:NamedIndividual, ns0:Industrial_oven ;
  rdfs:comment "Oven5 (Individual): an Industrial_oven"@en .

ns0:Particle_publish1
  a owl:NamedIndividual, ns0:Firmware ;
  ns0:send ns0:Cloud_Photon1 ;
  ns0:hasTimeLimit 30 ;
  rdfs:comment "Particle_publish1 (Individual): a Firmware with Object property assertions (send), Data property assertions (hasTimeLimit)"@en .

ns0:Particle_publish2
  a owl:NamedIndividual, ns0:Firmware ;
  ns0:send ns0:Cloud_Photon2 ;
  ns0:hasTimeLimit 25 ;
  rdfs:comment "Particle_publish2 (Individual): a Firmware with Object property assertions (send), Data property assertions (hasTimeLimit)"@en .

ns0:Paxos
  a owl:NamedIndividual, ns0:Data_center ;
  ns0:isApplied ns0:DC1, ns0:DC3, ns0:DC4 ;
  rdfs:comment "Paxos (Individual): a Data center with Object property assertions (isApplied)"@en .

ns0:Photon1
  a owl:NamedIndividual, ns0:Particle_Photon ;
  ns0:wire ns0:Connection1 ;
  rdfs:comment "Photon1 (Individual): a Particle_Photon with Object property assertions (wire)"@en .

ns0:Photon2
  a owl:NamedIndividual, ns0:Particle_Photon ;
  ns0:wire ns0:Connection2 ;
  rdfs:comment "Photon2 (Individual): a Particle_Photon with Object property assertions (wire)"@en .

ns0:Predictive_maintenance
  a owl:NamedIndividual, ns0:Edge_application ;
  ns0:hasTechnology ns0:OPC_servers ;
  rdfs:comment "Predictive_maintenance (Individual): an Edge application with Object property assertions (hasTechnology)"@en .

ns0:RTD3
  a owl:NamedIndividual, ns0:RTD_sensor ;
  ns0:heat ns0:Oven3 ;
  ns0:hasAccuracy "0.6"^^xsd:float ;
  ns0:provideHeat 5.100000e+2 ;
  rdfs:comment "RTD3 (Individual): an RTD_sensor with Object property assertions (heat), Data property assertions (provideHeat, hasAccuracy)"@en .

ns0:RTD4
  a owl:NamedIndividual, ns0:RTD_sensor ;
  ns0:heat ns0:Oven4 ;
  ns0:hasAccuracy "0.8"^^xsd:float ;
  ns0:provideHeat 5.200000e+2 ;
  rdfs:comment "RTD4 (Individual): an RTD_sensor with Object property assertions (heat), Data property assertions (provideHeat, hasAccuracy)"@en .

ns0:RTD5
  a owl:NamedIndividual, ns0:RTD_sensor ;
  ns0:heat ns0:Oven5 ;
  rdfs:comment "RTD5 (Individual): an RTD_sensor with Object property assertions (heat)"@en .

ns0:RTDsensor1
  a owl:NamedIndividual, ns0:RTD_sensor ;
  ns0:heat ns0:Oven1 ;
  ns0:hasAccuracy "0.5"^^xsd:float ;
  ns0:provideHeat 4.800000e+2 ;
  rdfs:comment "RTDsensor1 (Individual): an RTD_sensor with Object property assertions (heat), Data property assertions (provideHeat, hasAccuracy)"@en .

ns0:RTDsensor2
  a owl:NamedIndividual, ns0:RTD_sensor ;
  ns0:heat ns0:Oven2 ;
  ns0:hasAccuracy "0.3"^^xsd:float ;
  ns0:provideHeat 5.000000e+2 ;
  rdfs:comment "RTDsensor2 (Individual): an RTD_sensor with Object property assertions (heat), Data property assertions (provideHeat, hasAccuracy)"@en .

ns0:Reducing_latency_in_sending_data
  a owl:NamedIndividual, ns0:Blockchain_solution ;
  rdfs:comment "Reducing_latency_in_sending_data (Individual): a Blockchain solution"@en .

ns0:SCADA_application
  a owl:NamedIndividual, ns0:SCADA ;
  ns0:threats_to_data_security ns0:Data_security_risk ;
  rdfs:comment "SCADA_application (Individual): of SCADA type with Object property assertions (threats_to_data_security)"@en .

ns0:SCADA_system
  a owl:NamedIndividual, ns0:SCADA ;
  rdfs:comment "SCADA_system (Individual): of SCADA type"@en .

ns0:Secure_key_management
  a owl:NamedIndividual, ns0:Blockchain_solution ;
  rdfs:comment "Secure_key_management (Individual): a Blockchain solution"@en .

ns0:Security_problem
  a owl:NamedIndividual, ns0:Blockchain_security ;
  ns0:hasSolution ns0:Access_control, ns0:Data_protection, ns0:Integrity_assurance, ns0:Secure_key_management ;
  rdfs:comment "Security_problem (Individual): a Blockchain security type with Object property assertions (hasSolution)"@en .

ns0:Smart_contracts
  a owl:NamedIndividual, ns0:Blockchain ;
  ns0:hasSecurity_problem ns0:Security_problem ;
  rdfs:comment "Smart_contracts (Individual): of Blockchain type with Object property assertions (hasSecurity)"@en .

ns0:Smart_grid
  a owl:NamedIndividual, ns0:Edge_application ;
  ns0:hasTechnology ns0:OPC_servers ;
  rdfs:comment "Smart_grid (Individual): an Edge application with Object property assertions (hasTechnology)"@en .

ns0:Smart_home
  a owl:NamedIndividual, ns0:Edge_application ;
  ns0:hasTechnology ns0:OPC_servers ;
  rdfs:comment "Smart_home (Individual): an Edge application with Object property assertions (hasTechnology)"@en .

ns0:Strong_authentication
  a owl:NamedIndividual, ns0:SCADA_solution ;
  rdfs:comment "Strong_authentication (Object property): a SCADA_solution"@en .

ns0:Synchronization_in_throughput
  a owl:NamedIndividual, ns0:Blockchain_solution ;
  rdfs:comment "Synchronization_in_throughput (Individual): a Blockchain solution"@en .

ns0:TCP_IP
  a owl:NamedIndividual, ns0:SCADA_today_protocol ;
  ns0:Support_communication ns0:Long-distance_communication ;
  rdfs:comment "TCP_IP (Individual): a SCADA today protocol with Object property assertions (Support_communication)"@en .

ns0:Tensor_Flow
  a owl:NamedIndividual, ns0:Tool ;
  ns0:isToolFor ns0:Deep_learning_algorithm ;
  rdfs:comment "Tensor_Flow (Individual): a Tool with Object property assertions (isToolFor)"@en .

ns0:Theano
  a owl:NamedIndividual, ns0:Tool ;
  ns0:isToolFor ns0:Deep_learning_algorithm ;
  rdfs:comment "Theano (Individual): a Tool with Object property assertions (isToolFor)"@en .

ns0:Thingspeak1
  a owl:NamedIndividual, ns0:Subscriber ;
  rdfs:comment "Thingspeak1 (Individual): a Subscriber"@en .

ns0:Thingspeak2
  a owl:NamedIndividual, ns0:Subscriber ;
  rdfs:comment "Thingspeak2 (Individual): a Subscriber"@en .

ns0:Threats_at_critical_infrastructure
  a owl:NamedIndividual, ns0:SCADA_problem ;
  rdfs:comment "Threats_at_critical_infrastructure (Individual): a SCADA problem"@en .

ns0:Throughput_limited
  a owl:NamedIndividual, ns0:Blockchain_problem ;
  ns0:hasSolution ns0:Synchronization_in_throughput ;
  rdfs:comment "Throughput_limited (Individual): a Blockchain problem with Object property assertions (hasSolution)"@en .

ns0:Transmission_speed
  a owl:NamedIndividual, ns0:Edge_security ;
  ns0:best_Practices ns0:Smart_home ;
  ns0:has_SecuritySolution ns0:Reducing_latency_in_sending_data ;
  rdfs:comment "Transmission_speed (Individual): of Edge security type with Object property assertions (has_SecuritySolution, best_Practices)"@en .

ns0:Zookeeper
  a owl:NamedIndividual, ns0:Data_center ;
  ns0:hasService ns0:Maintain_configuration ;
  ns0:isApplied ns0:DC2 ;
  rdfs:comment "Zookeeper (Individual): a Data center with Object property assertions (isApplied, hasService)"@en .

owl:Thing
  rdfs:comment "IoT-TTA is a semantic ontology for Internet of Things technologies, tools, and applications."@en ;
  rdfs:seeAlso """Authors: Liviana N. Tudor, Lecia Barker, Mohammad Q. Azhar, Jorge Guerra, Clark Mousaw
Editor: Liviana N. Tudor"""@en .

<https://w3id.org/iot-tta/IoT-WG/ontologies/2022/3/IIoT#y> a <http://www.w3.org/2003/11/swrl#Variable> .
<https://w3id.org/iot-tta/IoT-WG/ontologies/2022/3/IIoT#x> a <http://www.w3.org/2003/11/swrl#Variable> .
<https://w3id.org/iot-tta/IoT-WG/ontologies/2022/3/IIoT#z> a <http://www.w3.org/2003/11/swrl#Variable> .
ns0:x a <http://www.w3.org/2003/11/swrl#Variable> .
ns0:z a <http://www.w3.org/2003/11/swrl#Variable> .
ns0:y a <http://www.w3.org/2003/11/swrl#Variable> .
<https://w3id.org/iot-tta/IoT-WG/ontologies/2022/3/IIoT#w> a <http://www.w3.org/2003/11/swrl#Variable> .
<https://w3id.org/iot-tta/IoT-WG/ontologies/2022/3/IIoT#q> a <http://www.w3.org/2003/11/swrl#Variable> .
<https://w3id.org/iot-tta/IoT-WG/ontologies/2022/3/IIoT#t> a <http://www.w3.org/2003/11/swrl#Variable> .
<https://w3id.org/iot-tta/IoT-WG/ontologies/2022/3/IIoT#s> a <http://www.w3.org/2003/11/swrl#Variable> .
_:genid3 xsd:minInclusive 20 .
_:genid5 xsd:maxInclusive 32 .
_:genid9 xsd:minInclusive 8.000000e+0 .
_:genid14 xsd:minInclusive "3.0"^^xsd:float .
_:genid18 xsd:minInclusive 2 .
_:genid22 xsd:maxInclusive 1 .
_:genid26 xsd:minInclusive "0.1"^^xsd:float .
_:genid28 xsd:maxInclusive "1.0"^^xsd:float .
_:genid32 xsd:minInclusive 5.000000e+2 .
_:genid34 xsd:maxInclusive 5.100000e+2 .
_:genid38 xsd:minInclusive 29 .
_:genid40 xsd:maxInclusive 30 .
_:genid44 xsd:minInclusive 0 .
_:genid46 xsd:maxInclusive 1 .
_:genid49
  a owl:Restriction ;
  owl:onProperty ns0:languages_tools ;
  owl:hasValue "C" .

_:genid51
  a owl:Restriction ;
  owl:onProperty ns0:languages_tools ;
  owl:hasValue "C++" .

_:genid53
  a owl:Restriction ;
  owl:onProperty ns0:languages_tools ;
  owl:hasValue "Cosm" .

_:genid55
  a owl:Restriction ;
  owl:onProperty ns0:languages_tools ;
  owl:hasValue "Ladder Logic" .

_:genid57
  a owl:Restriction ;
  owl:onProperty ns0:languages_tools ;
  owl:hasValue "Nimbits" .

_:genid59
  a owl:Restriction ;
  owl:onProperty ns0:languages_tools ;
  owl:hasValue "Python" .

_:genid61
  a owl:Restriction ;
  owl:onProperty ns0:languages_tools ;
  owl:hasValue "Wyliodrin Studio" .

_:genid64
  a owl:Restriction ;
  owl:onProperty ns0:operating_system ;
  owl:hasValue "Android" .

_:genid66
  a owl:Restriction ;
  owl:onProperty ns0:operating_system ;
  owl:hasValue "Linux" .

_:genid68
  a owl:Restriction ;
  owl:onProperty ns0:operating_system ;
  owl:hasValue "Mac" .

_:genid70
  a owl:Restriction ;
  owl:onProperty ns0:operating_system ;
  owl:hasValue "RaspberryPi" .

_:genid72
  a owl:Restriction ;
  owl:onProperty ns0:operating_system ;
  owl:hasValue "Raspbian" .

_:genid74
  a owl:Restriction ;
  owl:onProperty ns0:operating_system ;
  owl:hasValue "Windows" .

_:genid78 xsd:minInclusive -2.000000e+2 .
_:genid80 xsd:maxInclusive 6.000000e+2 .
[]
  a owl:AllDisjointClasses ;
  owl:members (
   ns0:Algorithm
   ns0:Programming_Language
   ns0:Web_Technology
 ) .

[]
  a owl:AllDisjointClasses ;
  owl:members (
   ns0:Application
   ns0:Capabilities
   ns0:Device
   ns0:Network
   ns0:Support
 ) .

[]
  a owl:AllDisjointClasses ;
  owl:members (
   ns0:Arduino
   ns0:Particle_Photon
   ns0:Raspberry_Pi
 ) .

[]
  a owl:AllDisjointClasses ;
  owl:members (
   ns0:BLE
   ns0:HTTP
   ns0:IP
   ns0:LoWPAN
   ns0:MQTT
   ns0:NFC_tag
   ns0:Optical_tag
   ns0:PAN
   ns0:RFID_tag
   ns0:SAMPL
   ns0:TCP
   ns0:UDP
   ns0:WPAN
   ns0:XMPP
 ) .

[]
  a owl:AllDisjointClasses ;
  owl:members (
   ns0:BigData_app
   ns0:Machine_learning
   ns0:SOA
   ns0:Web_socket
 ) .

[]
  a owl:AllDisjointClasses ;
  owl:members (
   ns0:C
   ns0:Java
   ns0:Python
 ) .

[]
  a owl:AllDisjointClasses ;
  owl:members (
   ns0:Computer_architecture
   ns0:Control_engineering
   ns0:Data_transmission
 ) .

[]
  a owl:AllDisjointClasses ;
  owl:members (
   ns0:Control_System
   ns0:Electrical_Grids
   ns0:Factory_Equipment
   ns0:Factory_Floor
   ns0:Gas_Meter
   ns0:Oil_Pipeline_Control
 ) .

[]
  a owl:AllDisjointClasses ;
  owl:members (
   ns0:Digital
   ns0:Gateway
   ns0:Sensor_Actuator
 ) .

[]
  a owl:AllDisjointClasses ;
  owl:members (
   ns0:Ethics
   ns0:Management
   ns0:Privacy
   ns0:Security
 ) .

[]
  a owl:AllDisjointClasses ;
  owl:members (
   ns0:Hardware_Platform
   ns0:Logic
   ns0:Purpose-built_Device
   ns0:Smart_Product
 ) .

[]
  a owl:AllDisjointClasses ;
  owl:members (
   ns0:Mahout
   ns0:Mllib
   ns0:Spark
 ) .

[]
  a owl:AllDifferent ;
  owl:distinctMembers (
   ns0:Particle_publish1
   ns0:Particle_publish2
 ) .

[]
  a owl:AllDifferent ;
  owl:distinctMembers (
   ns0:Thingspeak1
   ns0:Thingspeak2
 ) .

[]
  ns1:isRuleEnabled true ;
  rdfs:comment ""@en ;
  rdfs:label "R9a-a"@en ;
  a <http://www.w3.org/2003/11/swrl#Imp> ;
  ns2:body (
   _:genid157
   _:genid159
   _:genid161
   _:genid163
 ) ;
  ns2:head ( _:genid165 ) .

_:genid157
  a ns2:ClassAtom ;
  ns2:classPredicate ns0:Edge_technology ;
  ns2:argument1 <https://w3id.org/iot-tta/IoT-WG/ontologies/2022/3/IIoT#y> .

_:genid159
  a ns2:ClassAtom ;
  ns2:classPredicate ns0:Application ;
  ns2:argument1 <https://w3id.org/iot-tta/IoT-WG/ontologies/2022/3/IIoT#x> .

_:genid161
  a ns2:IndividualPropertyAtom ;
  ns2:propertyPredicate ns0:hasTool ;
  ns2:argument1 <https://w3id.org/iot-tta/IoT-WG/ontologies/2022/3/IIoT#y> ;
  ns2:argument2 <https://w3id.org/iot-tta/IoT-WG/ontologies/2022/3/IIoT#z> .

_:genid163
  a ns2:IndividualPropertyAtom ;
  ns2:propertyPredicate ns0:hasTechnology ;
  ns2:argument1 <https://w3id.org/iot-tta/IoT-WG/ontologies/2022/3/IIoT#x> ;
  ns2:argument2 <https://w3id.org/iot-tta/IoT-WG/ontologies/2022/3/IIoT#y> .

_:genid165
  a ns2:IndividualPropertyAtom ;
  ns2:propertyPredicate ns0:supporting_tool ;
  ns2:argument1 <https://w3id.org/iot-tta/IoT-WG/ontologies/2022/3/IIoT#x> ;
  ns2:argument2 <https://w3id.org/iot-tta/IoT-WG/ontologies/2022/3/IIoT#z> .

[]
  ns1:isRuleEnabled true ;
  rdfs:comment ""@en ;
  rdfs:label "R9a-b"@en ;
  a ns2:Imp ;
  ns2:body (
   _:genid168
   _:genid170
   _:genid172
   _:genid174
 ) ;
  ns2:head ( _:genid176 ) .

_:genid168
  a ns2:ClassAtom ;
  ns2:classPredicate ns0:Edge_technology ;
  ns2:argument1 <https://w3id.org/iot-tta/IoT-WG/ontologies/2022/3/IIoT#y> .

_:genid170
  a ns2:ClassAtom ;
  ns2:classPredicate ns0:Application ;
  ns2:argument1 <https://w3id.org/iot-tta/IoT-WG/ontologies/2022/3/IIoT#x> .

_:genid172
  a ns2:IndividualPropertyAtom ;
  ns2:propertyPredicate ns0:hasTool ;
  ns2:argument1 <https://w3id.org/iot-tta/IoT-WG/ontologies/2022/3/IIoT#y> ;
  ns2:argument2 <https://w3id.org/iot-tta/IoT-WG/ontologies/2022/3/IIoT#z> .

_:genid174
  a ns2:IndividualPropertyAtom ;
  ns2:propertyPredicate ns0:hasTechnology ;
  ns2:argument1 <https://w3id.org/iot-tta/IoT-WG/ontologies/2022/3/IIoT#x> ;
  ns2:argument2 <https://w3id.org/iot-tta/IoT-WG/ontologies/2022/3/IIoT#y> .

_:genid176
  a ns2:BuiltinAtom ;
  ns2:builtin <http://sqwrl.stanford.edu/ontologies/built-ins/3.4/sqwrl.owl#select> ;
  ns2:arguments (
   <https://w3id.org/iot-tta/IoT-WG/ontologies/2022/3/IIoT#x>
   <https://w3id.org/iot-tta/IoT-WG/ontologies/2022/3/IIoT#y>
   <https://w3id.org/iot-tta/IoT-WG/ontologies/2022/3/IIoT#z>
 ) .

[]
  ns1:isRuleEnabled true ;
  rdfs:comment ""@en ;
  rdfs:label "R4s-a"@en ;
  a ns2:Imp ;
  ns2:body (
   _:genid182
   _:genid184
   _:genid186
   _:genid188
 ) ;
  ns2:head ( _:genid190 ) .

_:genid182
  a ns2:IndividualPropertyAtom ;
  ns2:propertyPredicate ns0:isProcessed ;
  ns2:argument1 <https://w3id.org/iot-tta/IoT-WG/ontologies/2022/3/IIoT#y> ;
  ns2:argument2 <https://w3id.org/iot-tta/IoT-WG/ontologies/2022/3/IIoT#z> .

_:genid184
  a ns2:ClassAtom ;
  ns2:classPredicate ns0:Tool ;
  ns2:argument1 ns0:Apache_Hadoop .

_:genid186
  a ns2:IndividualPropertyAtom ;
  ns2:propertyPredicate ns0:isToolFor ;
  ns2:argument1 <https://w3id.org/iot-tta/IoT-WG/ontologies/2022/3/IIoT#x> ;
  ns2:argument2 <https://w3id.org/iot-tta/IoT-WG/ontologies/2022/3/IIoT#y> .

_:genid188
  a ns2:ClassAtom ;
  ns2:classPredicate ns0:BigData_capability ;
  ns2:argument1 <https://w3id.org/iot-tta/IoT-WG/ontologies/2022/3/IIoT#z> .

_:genid190
  a ns2:IndividualPropertyAtom ;
  ns2:propertyPredicate ns0:hasCapability ;
  ns2:argument1 <https://w3id.org/iot-tta/IoT-WG/ontologies/2022/3/IIoT#x> ;
  ns2:argument2 <https://w3id.org/iot-tta/IoT-WG/ontologies/2022/3/IIoT#z> .

[]
  ns1:isRuleEnabled true ;
  rdfs:comment ""@en ;
  rdfs:label "R4s-b"@en ;
  a ns2:Imp ;
  ns2:body (
   _:genid193
   _:genid195
   _:genid197
 ) ;
  ns2:head ( _:genid199 ) .

_:genid193
  a ns2:IndividualPropertyAtom ;
  ns2:propertyPredicate ns0:isProcessed ;
  ns2:argument1 <https://w3id.org/iot-tta/IoT-WG/ontologies/2022/3/IIoT#y> ;
  ns2:argument2 <https://w3id.org/iot-tta/IoT-WG/ontologies/2022/3/IIoT#z> .

_:genid195
  a ns2:IndividualPropertyAtom ;
  ns2:propertyPredicate ns0:isToolFor ;
  ns2:argument1 ns0:Apache_Hadoop ;
  ns2:argument2 <https://w3id.org/iot-tta/IoT-WG/ontologies/2022/3/IIoT#y> .

_:genid197
  a ns2:ClassAtom ;
  ns2:classPredicate ns0:BigData_capability ;
  ns2:argument1 <https://w3id.org/iot-tta/IoT-WG/ontologies/2022/3/IIoT#z> .

_:genid199
  a ns2:BuiltinAtom ;
  ns2:builtin <http://sqwrl.stanford.edu/ontologies/built-ins/3.4/sqwrl.owl#select> ;
  ns2:arguments (
   <https://w3id.org/iot-tta/IoT-WG/ontologies/2022/3/IIoT#y>
   <https://w3id.org/iot-tta/IoT-WG/ontologies/2022/3/IIoT#z>
 ) .

[]
  ns1:isRuleEnabled true ;
  rdfs:comment ""@en ;
  rdfs:label "R5a-a"@en ;
  a ns2:Imp ;
  ns2:body (
   _:genid204
   _:genid206
   _:genid208
   _:genid210
 ) ;
  ns2:head ( _:genid212 ) .

_:genid204
  a ns2:IndividualPropertyAtom ;
  ns2:propertyPredicate ns0:hasSolution ;
  ns2:argument1 <https://w3id.org/iot-tta/IoT-WG/ontologies/2022/3/IIoT#y> ;
  ns2:argument2 <https://w3id.org/iot-tta/IoT-WG/ontologies/2022/3/IIoT#z> .

_:genid206
  a ns2:ClassAtom ;
  ns2:classPredicate ns0:Blockchain ;
  ns2:argument1 <https://w3id.org/iot-tta/IoT-WG/ontologies/2022/3/IIoT#x> .

_:genid208
  a ns2:ClassAtom ;
  ns2:classPredicate ns0:Blockchain_problem ;
  ns2:argument1 <https://w3id.org/iot-tta/IoT-WG/ontologies/2022/3/IIoT#y> .

_:genid210
  a ns2:IndividualPropertyAtom ;
  ns2:propertyPredicate ns0:hasProblem ;
  ns2:argument1 <https://w3id.org/iot-tta/IoT-WG/ontologies/2022/3/IIoT#x> ;
  ns2:argument2 <https://w3id.org/iot-tta/IoT-WG/ontologies/2022/3/IIoT#y> .

_:genid212
  a ns2:IndividualPropertyAtom ;
  ns2:propertyPredicate ns0:challenge ;
  ns2:argument1 <https://w3id.org/iot-tta/IoT-WG/ontologies/2022/3/IIoT#x> ;
  ns2:argument2 <https://w3id.org/iot-tta/IoT-WG/ontologies/2022/3/IIoT#z> .

[]
  ns1:isRuleEnabled true ;
  rdfs:comment ""@en ;
  rdfs:label "R5a-b"@en ;
  a ns2:Imp ;
  ns2:body (
   _:genid215
   _:genid217
   _:genid219
   _:genid221
 ) ;
  ns2:head ( _:genid223 ) .

_:genid215
  a ns2:IndividualPropertyAtom ;
  ns2:propertyPredicate ns0:hasSolution ;
  ns2:argument1 <https://w3id.org/iot-tta/IoT-WG/ontologies/2022/3/IIoT#y> ;
  ns2:argument2 <https://w3id.org/iot-tta/IoT-WG/ontologies/2022/3/IIoT#z> .

_:genid217
  a ns2:ClassAtom ;
  ns2:classPredicate ns0:Blockchain ;
  ns2:argument1 <https://w3id.org/iot-tta/IoT-WG/ontologies/2022/3/IIoT#x> .

_:genid219
  a ns2:ClassAtom ;
  ns2:classPredicate ns0:Blockchain_problem ;
  ns2:argument1 <https://w3id.org/iot-tta/IoT-WG/ontologies/2022/3/IIoT#y> .

_:genid221
  a ns2:IndividualPropertyAtom ;
  ns2:propertyPredicate ns0:hasProblem ;
  ns2:argument1 <https://w3id.org/iot-tta/IoT-WG/ontologies/2022/3/IIoT#x> ;
  ns2:argument2 <https://w3id.org/iot-tta/IoT-WG/ontologies/2022/3/IIoT#y> .

_:genid223
  a ns2:BuiltinAtom ;
  ns2:builtin <http://sqwrl.stanford.edu/ontologies/built-ins/3.4/sqwrl.owl#select> ;
  ns2:arguments (
   <https://w3id.org/iot-tta/IoT-WG/ontologies/2022/3/IIoT#x>
   <https://w3id.org/iot-tta/IoT-WG/ontologies/2022/3/IIoT#y>
   <https://w3id.org/iot-tta/IoT-WG/ontologies/2022/3/IIoT#z>
 ) .

[]
  ns1:isRuleEnabled true ;
  rdfs:comment ""@en ;
  rdfs:label "R6a-b"@en ;
  a ns2:Imp ;
  ns2:body (
   _:genid229
   _:genid231
   _:genid233
   _:genid235
 ) ;
  ns2:head ( _:genid237 ) .

_:genid229
  a ns2:IndividualPropertyAtom ;
  ns2:propertyPredicate ns0:hasSolution ;
  ns2:argument1 <https://w3id.org/iot-tta/IoT-WG/ontologies/2022/3/IIoT#y> ;
  ns2:argument2 <https://w3id.org/iot-tta/IoT-WG/ontologies/2022/3/IIoT#z> .

_:genid231
  a ns2:ClassAtom ;
  ns2:classPredicate ns0:Blockchain ;
  ns2:argument1 <https://w3id.org/iot-tta/IoT-WG/ontologies/2022/3/IIoT#x> .

_:genid233
  a ns2:IndividualPropertyAtom ;
  ns2:propertyPredicate ns0:hasSecurity_problem ;
  ns2:argument1 <https://w3id.org/iot-tta/IoT-WG/ontologies/2022/3/IIoT#x> ;
  ns2:argument2 <https://w3id.org/iot-tta/IoT-WG/ontologies/2022/3/IIoT#y> .

_:genid235
  a ns2:ClassAtom ;
  ns2:classPredicate ns0:Blockchain_security ;
  ns2:argument1 <https://w3id.org/iot-tta/IoT-WG/ontologies/2022/3/IIoT#y> .

_:genid237
  a ns2:BuiltinAtom ;
  ns2:builtin <http://sqwrl.stanford.edu/ontologies/built-ins/3.4/sqwrl.owl#select> ;
  ns2:arguments (
   <https://w3id.org/iot-tta/IoT-WG/ontologies/2022/3/IIoT#x>
   <https://w3id.org/iot-tta/IoT-WG/ontologies/2022/3/IIoT#y>
   <https://w3id.org/iot-tta/IoT-WG/ontologies/2022/3/IIoT#z>
 ) .

[]
  ns1:isRuleEnabled true ;
  rdfs:comment ""@en ;
  rdfs:label "R6a-a"@en ;
  a ns2:Imp ;
  ns2:body (
   _:genid243
   _:genid245
   _:genid247
 ) ;
  ns2:head ( _:genid249 ) .

_:genid243
  a ns2:IndividualPropertyAtom ;
  ns2:propertyPredicate ns0:hasSolution ;
  ns2:argument1 <https://w3id.org/iot-tta/IoT-WG/ontologies/2022/3/IIoT#y> ;
  ns2:argument2 <https://w3id.org/iot-tta/IoT-WG/ontologies/2022/3/IIoT#z> .

_:genid245
  a ns2:IndividualPropertyAtom ;
  ns2:propertyPredicate ns0:hasSecurity_problem ;
  ns2:argument1 ns0:Smart_contracts ;
  ns2:argument2 <https://w3id.org/iot-tta/IoT-WG/ontologies/2022/3/IIoT#y> .

_:genid247
  a ns2:ClassAtom ;
  ns2:classPredicate ns0:Blockchain ;
  ns2:argument1 <https://w3id.org/iot-tta/IoT-WG/ontologies/2022/3/IIoT#x> .

_:genid249
  a ns2:IndividualPropertyAtom ;
  ns2:propertyPredicate ns0:challenge ;
  ns2:argument1 <https://w3id.org/iot-tta/IoT-WG/ontologies/2022/3/IIoT#x> ;
  ns2:argument2 <https://w3id.org/iot-tta/IoT-WG/ontologies/2022/3/IIoT#z> .

[]
  ns1:isRuleEnabled true ;
  rdfs:comment ""@en ;
  rdfs:label "R10a-a"@en ;
  a ns2:Imp ;
  ns2:body (
   _:genid252
   _:genid254
   _:genid256
   _:genid258
 ) ;
  ns2:head ( _:genid260 ) .

_:genid252
  a ns2:IndividualPropertyAtom ;
  ns2:propertyPredicate ns0:best_Practices ;
  ns2:argument1 <https://w3id.org/iot-tta/IoT-WG/ontologies/2022/3/IIoT#x> ;
  ns2:argument2 <https://w3id.org/iot-tta/IoT-WG/ontologies/2022/3/IIoT#z> .

_:genid254
  a ns2:IndividualPropertyAtom ;
  ns2:propertyPredicate ns0:has_SecuritySolution ;
  ns2:argument1 <https://w3id.org/iot-tta/IoT-WG/ontologies/2022/3/IIoT#x> ;
  ns2:argument2 <https://w3id.org/iot-tta/IoT-WG/ontologies/2022/3/IIoT#y> .

_:genid256
  a ns2:ClassAtom ;
  ns2:classPredicate ns0:Edge_security ;
  ns2:argument1 <https://w3id.org/iot-tta/IoT-WG/ontologies/2022/3/IIoT#x> .

_:genid258
  a ns2:ClassAtom ;
  ns2:classPredicate ns0:Blockchain_solution ;
  ns2:argument1 <https://w3id.org/iot-tta/IoT-WG/ontologies/2022/3/IIoT#y> .

_:genid260
  a ns2:IndividualPropertyAtom ;
  ns2:propertyPredicate ns0:DevelopEdgeSecurity ;
  ns2:argument1 <https://w3id.org/iot-tta/IoT-WG/ontologies/2022/3/IIoT#z> ;
  ns2:argument2 <https://w3id.org/iot-tta/IoT-WG/ontologies/2022/3/IIoT#y> .

[]
  ns1:isRuleEnabled true ;
  rdfs:comment ""@en ;
  rdfs:label "R10a-b"@en ;
  a ns2:Imp ;
  ns2:body (
   _:genid263
   _:genid265
   _:genid267
   _:genid269
 ) ;
  ns2:head ( _:genid271 ) .

_:genid263
  a ns2:IndividualPropertyAtom ;
  ns2:propertyPredicate ns0:best_Practices ;
  ns2:argument1 <https://w3id.org/iot-tta/IoT-WG/ontologies/2022/3/IIoT#x> ;
  ns2:argument2 <https://w3id.org/iot-tta/IoT-WG/ontologies/2022/3/IIoT#z> .

_:genid265
  a ns2:IndividualPropertyAtom ;
  ns2:propertyPredicate ns0:has_SecuritySolution ;
  ns2:argument1 <https://w3id.org/iot-tta/IoT-WG/ontologies/2022/3/IIoT#x> ;
  ns2:argument2 <https://w3id.org/iot-tta/IoT-WG/ontologies/2022/3/IIoT#y> .

_:genid267
  a ns2:ClassAtom ;
  ns2:classPredicate ns0:Edge_security ;
  ns2:argument1 <https://w3id.org/iot-tta/IoT-WG/ontologies/2022/3/IIoT#x> .

_:genid269
  a ns2:ClassAtom ;
  ns2:classPredicate ns0:Blockchain_solution ;
  ns2:argument1 <https://w3id.org/iot-tta/IoT-WG/ontologies/2022/3/IIoT#y> .

_:genid271
  a ns2:BuiltinAtom ;
  ns2:builtin <http://sqwrl.stanford.edu/ontologies/built-ins/3.4/sqwrl.owl#select> ;
  ns2:arguments (
   <https://w3id.org/iot-tta/IoT-WG/ontologies/2022/3/IIoT#x>
   <https://w3id.org/iot-tta/IoT-WG/ontologies/2022/3/IIoT#y>
   <https://w3id.org/iot-tta/IoT-WG/ontologies/2022/3/IIoT#z>
 ) .

[]
  ns1:isRuleEnabled true ;
  rdfs:comment ""@en ;
  rdfs:label "R3sb"@en ;
  a ns2:Imp ;
  ns2:body (
   _:genid277
   _:genid279
   _:genid281
   _:genid283
 ) ;
  ns2:head ( _:genid285 ) .

_:genid277
  a ns2:IndividualPropertyAtom ;
  ns2:propertyPredicate ns0:useProgramming ;
  ns2:argument1 ns0:x ;
  ns2:argument2 ns0:z .

_:genid279
  a ns2:ClassAtom ;
  ns2:classPredicate ns0:Computer_cluster ;
  ns2:argument1 ns0:y .

_:genid281
  a ns2:ClassAtom ;
  ns2:classPredicate ns0:Tool ;
  ns2:argument1 ns0:x .

_:genid283
  a ns2:IndividualPropertyAtom ;
  ns2:propertyPredicate ns0:isToolFor ;
  ns2:argument1 ns0:x ;
  ns2:argument2 ns0:y .

_:genid285
  a ns2:BuiltinAtom ;
  ns2:builtin <http://sqwrl.stanford.edu/ontologies/built-ins/3.4/sqwrl.owl#select> ;
  ns2:arguments (
   ns0:x
   ns0:y
   ns0:z
 ) .

[]
  ns1:isRuleEnabled true ;
  rdfs:comment ""@en ;
  rdfs:label "R2s-a"@en ;
  a ns2:Imp ;
  ns2:body (
   _:genid291
   _:genid293
   _:genid295
 ) ;
  ns2:head ( _:genid297 ) .

_:genid291
  a ns2:IndividualPropertyAtom ;
  ns2:propertyPredicate ns0:hasService ;
  ns2:argument1 ns0:x ;
  ns2:argument2 ns0:y .

_:genid293
  a ns2:IndividualPropertyAtom ;
  ns2:propertyPredicate ns0:useAlgorithm ;
  ns2:argument1 ns0:x ;
  ns2:argument2 ns0:z .

_:genid295
  a ns2:ClassAtom ;
  ns2:classPredicate ns0:Data_center ;
  ns2:argument1 ns0:x .

_:genid297
  a ns2:IndividualPropertyAtom ;
  ns2:propertyPredicate ns0:hasFunctionality ;
  ns2:argument1 ns0:x ;
  ns2:argument2 ns0:y .

[]
  ns1:isRuleEnabled true ;
  rdfs:comment ""@en ;
  rdfs:label "R2s-b"@en ;
  a ns2:Imp ;
  ns2:body (
   _:genid300
   _:genid302
   _:genid304
 ) ;
  ns2:head ( _:genid306 ) .

_:genid300
  a ns2:IndividualPropertyAtom ;
  ns2:propertyPredicate ns0:hasService ;
  ns2:argument1 <https://w3id.org/iot-tta/IoT-WG/ontologies/2022/3/IIoT#x> ;
  ns2:argument2 <https://w3id.org/iot-tta/IoT-WG/ontologies/2022/3/IIoT#y> .

_:genid302
  a ns2:IndividualPropertyAtom ;
  ns2:propertyPredicate ns0:useAlgorithm ;
  ns2:argument1 <https://w3id.org/iot-tta/IoT-WG/ontologies/2022/3/IIoT#x> ;
  ns2:argument2 <https://w3id.org/iot-tta/IoT-WG/ontologies/2022/3/IIoT#z> .

_:genid304
  a ns2:ClassAtom ;
  ns2:classPredicate ns0:Data_center ;
  ns2:argument1 <https://w3id.org/iot-tta/IoT-WG/ontologies/2022/3/IIoT#x> .

_:genid306
  a ns2:BuiltinAtom ;
  ns2:builtin <http://sqwrl.stanford.edu/ontologies/built-ins/3.4/sqwrl.owl#select> ;
  ns2:arguments (
   <https://w3id.org/iot-tta/IoT-WG/ontologies/2022/3/IIoT#x>
   <https://w3id.org/iot-tta/IoT-WG/ontologies/2022/3/IIoT#y>
   <https://w3id.org/iot-tta/IoT-WG/ontologies/2022/3/IIoT#z>
 ) .

[]
  ns1:isRuleEnabled true ;
  rdfs:comment ""@en ;
  rdfs:label "R11c-a"@en ;
  a ns2:Imp ;
  ns2:body (
   _:genid312
   _:genid314
   _:genid316
   _:genid318
   _:genid320
   _:genid322
   _:genid324
   _:genid326
   _:genid328
   _:genid330
   _:genid332
 ) ;
  ns2:head ( _:genid334 ) .

_:genid312
  a ns2:DatavaluedPropertyAtom ;
  ns2:propertyPredicate ns0:hasTimeLimit ;
  ns2:argument1 <https://w3id.org/iot-tta/IoT-WG/ontologies/2022/3/IIoT#z> ;
  ns2:argument2 30 .

_:genid314
  a ns2:IndividualPropertyAtom ;
  ns2:propertyPredicate ns0:read ;
  ns2:argument1 <https://w3id.org/iot-tta/IoT-WG/ontologies/2022/3/IIoT#y> ;
  ns2:argument2 <https://w3id.org/iot-tta/IoT-WG/ontologies/2022/3/IIoT#z> .

_:genid316
  a ns2:ClassAtom ;
  ns2:classPredicate ns0:Particle_Photon ;
  ns2:argument1 <https://w3id.org/iot-tta/IoT-WG/ontologies/2022/3/IIoT#x> .

_:genid318
  a ns2:IndividualPropertyAtom ;
  ns2:propertyPredicate ns0:send ;
  ns2:argument1 <https://w3id.org/iot-tta/IoT-WG/ontologies/2022/3/IIoT#z> ;
  ns2:argument2 <https://w3id.org/iot-tta/IoT-WG/ontologies/2022/3/IIoT#w> .

_:genid320
  a ns2:IndividualPropertyAtom ;
  ns2:propertyPredicate ns0:wire ;
  ns2:argument1 <https://w3id.org/iot-tta/IoT-WG/ontologies/2022/3/IIoT#x> ;
  ns2:argument2 <https://w3id.org/iot-tta/IoT-WG/ontologies/2022/3/IIoT#y> .

_:genid322
  a ns2:ClassAtom ;
  ns2:classPredicate ns0:Flow ;
  ns2:argument1 <https://w3id.org/iot-tta/IoT-WG/ontologies/2022/3/IIoT#y> .

_:genid324
  a ns2:DatavaluedPropertyAtom ;
  ns2:propertyPredicate ns0:hasValueConnection ;
  ns2:argument1 <https://w3id.org/iot-tta/IoT-WG/ontologies/2022/3/IIoT#y> ;
  ns2:argument2 1 .

_:genid326
  a ns2:ClassAtom ;
  ns2:classPredicate ns0:Particle_cloud ;
  ns2:argument1 <https://w3id.org/iot-tta/IoT-WG/ontologies/2022/3/IIoT#w> .

_:genid328
  a ns2:ClassAtom ;
  ns2:classPredicate ns0:Firmware ;
  ns2:argument1 <https://w3id.org/iot-tta/IoT-WG/ontologies/2022/3/IIoT#z> .

_:genid330
  a ns2:IndividualPropertyAtom ;
  ns2:propertyPredicate ns0:request ;
  ns2:argument1 <https://w3id.org/iot-tta/IoT-WG/ontologies/2022/3/IIoT#w> ;
  ns2:argument2 <https://w3id.org/iot-tta/IoT-WG/ontologies/2022/3/IIoT#q> .

_:genid332
  a ns2:ClassAtom ;
  ns2:classPredicate ns0:Subscriber ;
  ns2:argument1 <https://w3id.org/iot-tta/IoT-WG/ontologies/2022/3/IIoT#q> .

_:genid334
  a ns2:IndividualPropertyAtom ;
  ns2:propertyPredicate ns0:flow_services ;
  ns2:argument1 <https://w3id.org/iot-tta/IoT-WG/ontologies/2022/3/IIoT#x> ;
  ns2:argument2 <https://w3id.org/iot-tta/IoT-WG/ontologies/2022/3/IIoT#q> .

[]
  ns1:isRuleEnabled true ;
  rdfs:comment ""@en ;
  rdfs:label "R11c-b"@en ;
  a ns2:Imp ;
  ns2:body (
   _:genid337
   _:genid339
   _:genid341
   _:genid343
   _:genid345
   _:genid347
   _:genid349
   _:genid351
   _:genid353
   _:genid355
   _:genid357
 ) ;
  ns2:head ( _:genid359 ) .

_:genid337
  a ns2:DatavaluedPropertyAtom ;
  ns2:propertyPredicate ns0:hasTimeLimit ;
  ns2:argument1 <https://w3id.org/iot-tta/IoT-WG/ontologies/2022/3/IIoT#z> ;
  ns2:argument2 30 .

_:genid339
  a ns2:IndividualPropertyAtom ;
  ns2:propertyPredicate ns0:read ;
  ns2:argument1 <https://w3id.org/iot-tta/IoT-WG/ontologies/2022/3/IIoT#y> ;
  ns2:argument2 <https://w3id.org/iot-tta/IoT-WG/ontologies/2022/3/IIoT#z> .

_:genid341
  a ns2:ClassAtom ;
  ns2:classPredicate ns0:Particle_Photon ;
  ns2:argument1 <https://w3id.org/iot-tta/IoT-WG/ontologies/2022/3/IIoT#x> .

_:genid343
  a ns2:IndividualPropertyAtom ;
  ns2:propertyPredicate ns0:send ;
  ns2:argument1 <https://w3id.org/iot-tta/IoT-WG/ontologies/2022/3/IIoT#z> ;
  ns2:argument2 <https://w3id.org/iot-tta/IoT-WG/ontologies/2022/3/IIoT#w> .

_:genid345
  a ns2:IndividualPropertyAtom ;
  ns2:propertyPredicate ns0:wire ;
  ns2:argument1 <https://w3id.org/iot-tta/IoT-WG/ontologies/2022/3/IIoT#x> ;
  ns2:argument2 <https://w3id.org/iot-tta/IoT-WG/ontologies/2022/3/IIoT#y> .

_:genid347
  a ns2:ClassAtom ;
  ns2:classPredicate ns0:Flow ;
  ns2:argument1 <https://w3id.org/iot-tta/IoT-WG/ontologies/2022/3/IIoT#y> .

_:genid349
  a ns2:DatavaluedPropertyAtom ;
  ns2:propertyPredicate ns0:hasValueConnection ;
  ns2:argument1 <https://w3id.org/iot-tta/IoT-WG/ontologies/2022/3/IIoT#y> ;
  ns2:argument2 1 .

_:genid351
  a ns2:ClassAtom ;
  ns2:classPredicate ns0:Particle_cloud ;
  ns2:argument1 <https://w3id.org/iot-tta/IoT-WG/ontologies/2022/3/IIoT#w> .

_:genid353
  a ns2:ClassAtom ;
  ns2:classPredicate ns0:Firmware ;
  ns2:argument1 <https://w3id.org/iot-tta/IoT-WG/ontologies/2022/3/IIoT#z> .

_:genid355
  a ns2:IndividualPropertyAtom ;
  ns2:propertyPredicate ns0:request ;
  ns2:argument1 <https://w3id.org/iot-tta/IoT-WG/ontologies/2022/3/IIoT#w> ;
  ns2:argument2 <https://w3id.org/iot-tta/IoT-WG/ontologies/2022/3/IIoT#q> .

_:genid357
  a ns2:ClassAtom ;
  ns2:classPredicate ns0:Subscriber ;
  ns2:argument1 <https://w3id.org/iot-tta/IoT-WG/ontologies/2022/3/IIoT#q> .

_:genid359
  a ns2:BuiltinAtom ;
  ns2:builtin <http://sqwrl.stanford.edu/ontologies/built-ins/3.4/sqwrl.owl#select> ;
  ns2:arguments (
   <https://w3id.org/iot-tta/IoT-WG/ontologies/2022/3/IIoT#x>
   <https://w3id.org/iot-tta/IoT-WG/ontologies/2022/3/IIoT#y>
   <https://w3id.org/iot-tta/IoT-WG/ontologies/2022/3/IIoT#z>
   <https://w3id.org/iot-tta/IoT-WG/ontologies/2022/3/IIoT#w>
   <https://w3id.org/iot-tta/IoT-WG/ontologies/2022/3/IIoT#q>
 ) .

[]
  ns1:isRuleEnabled true ;
  rdfs:comment ""@en ;
  rdfs:label "R12c-a"@en ;
  a ns2:Imp ;
  ns2:body (
   _:genid367
   _:genid369
   _:genid371
   _:genid375
   _:genid377
   _:genid381
   _:genid383
   _:genid385
 ) ;
  ns2:head ( _:genid387 ) .

_:genid367
  a ns2:DatavaluedPropertyAtom ;
  ns2:propertyPredicate ns0:hasTemperatureRange ;
  ns2:argument1 <https://w3id.org/iot-tta/IoT-WG/ontologies/2022/3/IIoT#y> ;
  ns2:argument2 <https://w3id.org/iot-tta/IoT-WG/ontologies/2022/3/IIoT#w> .

_:genid369
  a ns2:IndividualPropertyAtom ;
  ns2:propertyPredicate ns0:heat ;
  ns2:argument1 <https://w3id.org/iot-tta/IoT-WG/ontologies/2022/3/IIoT#x> ;
  ns2:argument2 <https://w3id.org/iot-tta/IoT-WG/ontologies/2022/3/IIoT#y> .

_:genid371
  a ns2:BuiltinAtom ;
  ns2:builtin <http://www.w3.org/2003/11/swrlb#greaterThan> ;
  ns2:arguments (
   <https://w3id.org/iot-tta/IoT-WG/ontologies/2022/3/IIoT#z>
   <https://w3id.org/iot-tta/IoT-WG/ontologies/2022/3/IIoT#w>
 ) .

_:genid375
  a ns2:ClassAtom ;
  ns2:classPredicate ns0:RTD_sensor ;
  ns2:argument1 <https://w3id.org/iot-tta/IoT-WG/ontologies/2022/3/IIoT#x> .

_:genid377
  a ns2:BuiltinAtom ;
  ns2:builtin <http://www.w3.org/2003/11/swrlb#greaterThan> ;
  ns2:arguments (
   <https://w3id.org/iot-tta/IoT-WG/ontologies/2022/3/IIoT#t>
   0.7
 ) .

_:genid381
  a ns2:DatavaluedPropertyAtom ;
  ns2:propertyPredicate ns0:hasAccuracy ;
  ns2:argument1 <https://w3id.org/iot-tta/IoT-WG/ontologies/2022/3/IIoT#x> ;
  ns2:argument2 <https://w3id.org/iot-tta/IoT-WG/ontologies/2022/3/IIoT#t> .

_:genid383
  a ns2:DatavaluedPropertyAtom ;
  ns2:propertyPredicate ns0:provideHeat ;
  ns2:argument1 <https://w3id.org/iot-tta/IoT-WG/ontologies/2022/3/IIoT#x> ;
  ns2:argument2 <https://w3id.org/iot-tta/IoT-WG/ontologies/2022/3/IIoT#z> .

_:genid385
  a ns2:ClassAtom ;
  ns2:classPredicate ns0:Industrial_oven ;
  ns2:argument1 <https://w3id.org/iot-tta/IoT-WG/ontologies/2022/3/IIoT#y> .

_:genid387
  a ns2:IndividualPropertyAtom ;
  ns2:propertyPredicate ns0:regulationTemperature ;
  ns2:argument1 <https://w3id.org/iot-tta/IoT-WG/ontologies/2022/3/IIoT#x> ;
  ns2:argument2 <https://w3id.org/iot-tta/IoT-WG/ontologies/2022/3/IIoT#y> .

[]
  ns1:isRuleEnabled true ;
  rdfs:comment ""@en ;
  rdfs:label "R12c-b"@en ;
  a ns2:Imp ;
  ns2:body (
   _:genid390
   _:genid392
   _:genid394
   _:genid398
   _:genid400
   _:genid404
   _:genid406
   _:genid408
 ) ;
  ns2:head ( _:genid410 ) .

_:genid390
  a ns2:DatavaluedPropertyAtom ;
  ns2:propertyPredicate ns0:hasTemperatureRange ;
  ns2:argument1 <https://w3id.org/iot-tta/IoT-WG/ontologies/2022/3/IIoT#y> ;
  ns2:argument2 <https://w3id.org/iot-tta/IoT-WG/ontologies/2022/3/IIoT#w> .

_:genid392
  a ns2:IndividualPropertyAtom ;
  ns2:propertyPredicate ns0:heat ;
  ns2:argument1 <https://w3id.org/iot-tta/IoT-WG/ontologies/2022/3/IIoT#x> ;
  ns2:argument2 <https://w3id.org/iot-tta/IoT-WG/ontologies/2022/3/IIoT#y> .

_:genid394
  a ns2:BuiltinAtom ;
  ns2:builtin <http://www.w3.org/2003/11/swrlb#greaterThan> ;
  ns2:arguments (
   <https://w3id.org/iot-tta/IoT-WG/ontologies/2022/3/IIoT#z>
   <https://w3id.org/iot-tta/IoT-WG/ontologies/2022/3/IIoT#w>
 ) .

_:genid398
  a ns2:ClassAtom ;
  ns2:classPredicate ns0:RTD_sensor ;
  ns2:argument1 <https://w3id.org/iot-tta/IoT-WG/ontologies/2022/3/IIoT#x> .

_:genid400
  a ns2:BuiltinAtom ;
  ns2:builtin <http://www.w3.org/2003/11/swrlb#greaterThan> ;
  ns2:arguments (
   <https://w3id.org/iot-tta/IoT-WG/ontologies/2022/3/IIoT#t>
   0.7
 ) .

_:genid404
  a ns2:DatavaluedPropertyAtom ;
  ns2:propertyPredicate ns0:hasAccuracy ;
  ns2:argument1 <https://w3id.org/iot-tta/IoT-WG/ontologies/2022/3/IIoT#x> ;
  ns2:argument2 <https://w3id.org/iot-tta/IoT-WG/ontologies/2022/3/IIoT#t> .

_:genid406
  a ns2:DatavaluedPropertyAtom ;
  ns2:propertyPredicate ns0:provideHeat ;
  ns2:argument1 <https://w3id.org/iot-tta/IoT-WG/ontologies/2022/3/IIoT#x> ;
  ns2:argument2 <https://w3id.org/iot-tta/IoT-WG/ontologies/2022/3/IIoT#z> .

_:genid408
  a ns2:ClassAtom ;
  ns2:classPredicate ns0:Industrial_oven ;
  ns2:argument1 <https://w3id.org/iot-tta/IoT-WG/ontologies/2022/3/IIoT#y> .

_:genid410
  a ns2:BuiltinAtom ;
  ns2:builtin <http://sqwrl.stanford.edu/ontologies/built-ins/3.4/sqwrl.owl#select> ;
  ns2:arguments (
   <https://w3id.org/iot-tta/IoT-WG/ontologies/2022/3/IIoT#x>
   <https://w3id.org/iot-tta/IoT-WG/ontologies/2022/3/IIoT#z>
   <https://w3id.org/iot-tta/IoT-WG/ontologies/2022/3/IIoT#y>
   <https://w3id.org/iot-tta/IoT-WG/ontologies/2022/3/IIoT#w>
   <https://w3id.org/iot-tta/IoT-WG/ontologies/2022/3/IIoT#t>
 ) .

[]
  ns1:isRuleEnabled true ;
  rdfs:comment ""@en ;
  rdfs:label "R7a-b"@en ;
  a ns2:Imp ;
  ns2:body (
   _:genid418
   _:genid420
   _:genid422
   _:genid424
   _:genid426
 ) ;
  ns2:head ( _:genid428 ) .

_:genid418
  a ns2:IndividualPropertyAtom ;
  ns2:propertyPredicate ns0:SCADA_hasCapability ;
  ns2:argument1 <https://w3id.org/iot-tta/IoT-WG/ontologies/2022/3/IIoT#s> ;
  ns2:argument2 <https://w3id.org/iot-tta/IoT-WG/ontologies/2022/3/IIoT#w> .

_:genid420
  a ns2:ClassAtom ;
  ns2:classPredicate ns0:SCADA ;
  ns2:argument1 <https://w3id.org/iot-tta/IoT-WG/ontologies/2022/3/IIoT#s> .

_:genid422
  a ns2:IndividualPropertyAtom ;
  ns2:propertyPredicate ns0:Protocols_were_layered ;
  ns2:argument1 <https://w3id.org/iot-tta/IoT-WG/ontologies/2022/3/IIoT#x> ;
  ns2:argument2 <https://w3id.org/iot-tta/IoT-WG/ontologies/2022/3/IIoT#z> .

_:genid424
  a ns2:IndividualPropertyAtom ;
  ns2:propertyPredicate ns0:Lack_security_measure ;
  ns2:argument1 <https://w3id.org/iot-tta/IoT-WG/ontologies/2022/3/IIoT#x> ;
  ns2:argument2 <https://w3id.org/iot-tta/IoT-WG/ontologies/2022/3/IIoT#y> .

_:genid426
  a ns2:IndividualPropertyAtom ;
  ns2:propertyPredicate ns0:Support_communication ;
  ns2:argument1 <https://w3id.org/iot-tta/IoT-WG/ontologies/2022/3/IIoT#z> ;
  ns2:argument2 <https://w3id.org/iot-tta/IoT-WG/ontologies/2022/3/IIoT#w> .

_:genid428
  a ns2:BuiltinAtom ;
  ns2:builtin <http://sqwrl.stanford.edu/ontologies/built-ins/3.4/sqwrl.owl#select> ;
  ns2:arguments (
   <https://w3id.org/iot-tta/IoT-WG/ontologies/2022/3/IIoT#s>
   <https://w3id.org/iot-tta/IoT-WG/ontologies/2022/3/IIoT#x>
   <https://w3id.org/iot-tta/IoT-WG/ontologies/2022/3/IIoT#y>
   <https://w3id.org/iot-tta/IoT-WG/ontologies/2022/3/IIoT#z>
   <https://w3id.org/iot-tta/IoT-WG/ontologies/2022/3/IIoT#w>
 ) .

[]
  ns1:isRuleEnabled true ;
  rdfs:comment ""@en ;
  rdfs:label "R7a-a"@en ;
  a ns2:Imp ;
  ns2:body (
   _:genid436
   _:genid438
   _:genid440
   _:genid442
 ) ;
  ns2:head ( _:genid444 ) .

_:genid436
  a ns2:ClassAtom ;
  ns2:classPredicate ns0:SCADA ;
  ns2:argument1 <https://w3id.org/iot-tta/IoT-WG/ontologies/2022/3/IIoT#s> .

_:genid438
  a ns2:IndividualPropertyAtom ;
  ns2:propertyPredicate ns0:Protocols_were_layered ;
  ns2:argument1 <https://w3id.org/iot-tta/IoT-WG/ontologies/2022/3/IIoT#x> ;
  ns2:argument2 <https://w3id.org/iot-tta/IoT-WG/ontologies/2022/3/IIoT#z> .

_:genid440
  a ns2:IndividualPropertyAtom ;
  ns2:propertyPredicate ns0:Lack_security_measure ;
  ns2:argument1 <https://w3id.org/iot-tta/IoT-WG/ontologies/2022/3/IIoT#x> ;
  ns2:argument2 <https://w3id.org/iot-tta/IoT-WG/ontologies/2022/3/IIoT#y> .

_:genid442
  a ns2:IndividualPropertyAtom ;
  ns2:propertyPredicate ns0:Support_communication ;
  ns2:argument1 <https://w3id.org/iot-tta/IoT-WG/ontologies/2022/3/IIoT#z> ;
  ns2:argument2 <https://w3id.org/iot-tta/IoT-WG/ontologies/2022/3/IIoT#w> .

_:genid444
  a ns2:IndividualPropertyAtom ;
  ns2:propertyPredicate ns0:SCADA_hasCapability ;
  ns2:argument1 <https://w3id.org/iot-tta/IoT-WG/ontologies/2022/3/IIoT#s> ;
  ns2:argument2 <https://w3id.org/iot-tta/IoT-WG/ontologies/2022/3/IIoT#w> .

[]
  ns1:isRuleEnabled true ;
  rdfs:comment ""@en ;
  rdfs:label "R8a-a"@en ;
  a ns2:Imp ;
  ns2:body (
   _:genid447
   _:genid449
   _:genid451
 ) ;
  ns2:head ( _:genid453 ) .

_:genid447
  a ns2:IndividualPropertyAtom ;
  ns2:propertyPredicate ns0:threats_to_data_security ;
  ns2:argument1 <https://w3id.org/iot-tta/IoT-WG/ontologies/2022/3/IIoT#x> ;
  ns2:argument2 <https://w3id.org/iot-tta/IoT-WG/ontologies/2022/3/IIoT#y> .

_:genid449
  a ns2:ClassAtom ;
  ns2:classPredicate ns0:SCADA ;
  ns2:argument1 <https://w3id.org/iot-tta/IoT-WG/ontologies/2022/3/IIoT#x> .

_:genid451
  a ns2:IndividualPropertyAtom ;
  ns2:propertyPredicate ns0:countermeasure ;
  ns2:argument1 <https://w3id.org/iot-tta/IoT-WG/ontologies/2022/3/IIoT#y> ;
  ns2:argument2 <https://w3id.org/iot-tta/IoT-WG/ontologies/2022/3/IIoT#z> .

_:genid453
  a ns2:IndividualPropertyAtom ;
  ns2:propertyPredicate ns0:Dealing_with_sensitive_data ;
  ns2:argument1 <https://w3id.org/iot-tta/IoT-WG/ontologies/2022/3/IIoT#x> ;
  ns2:argument2 <https://w3id.org/iot-tta/IoT-WG/ontologies/2022/3/IIoT#z> .

[]
  ns1:isRuleEnabled true ;
  rdfs:comment ""@en ;
  rdfs:label "R8a-b"@en ;
  a ns2:Imp ;
  ns2:body (
   _:genid456
   _:genid458
   _:genid460
 ) ;
  ns2:head ( _:genid462 ) .

_:genid456
  a ns2:IndividualPropertyAtom ;
  ns2:propertyPredicate ns0:threats_to_data_security ;
  ns2:argument1 <https://w3id.org/iot-tta/IoT-WG/ontologies/2022/3/IIoT#x> ;
  ns2:argument2 <https://w3id.org/iot-tta/IoT-WG/ontologies/2022/3/IIoT#y> .

_:genid458
  a ns2:ClassAtom ;
  ns2:classPredicate ns0:SCADA ;
  ns2:argument1 <https://w3id.org/iot-tta/IoT-WG/ontologies/2022/3/IIoT#x> .

_:genid460
  a ns2:IndividualPropertyAtom ;
  ns2:propertyPredicate ns0:countermeasure ;
  ns2:argument1 <https://w3id.org/iot-tta/IoT-WG/ontologies/2022/3/IIoT#y> ;
  ns2:argument2 <https://w3id.org/iot-tta/IoT-WG/ontologies/2022/3/IIoT#z> .

_:genid462
  a ns2:BuiltinAtom ;
  ns2:builtin <http://sqwrl.stanford.edu/ontologies/built-ins/3.4/sqwrl.owl#select> ;
  ns2:arguments (
   <https://w3id.org/iot-tta/IoT-WG/ontologies/2022/3/IIoT#x>
   <https://w3id.org/iot-tta/IoT-WG/ontologies/2022/3/IIoT#y>
   <https://w3id.org/iot-tta/IoT-WG/ontologies/2022/3/IIoT#z>
 ) .

[]
  ns1:isRuleEnabled true ;
  rdfs:comment ""@en ;
  rdfs:label "R1s1"@en ;
  a ns2:Imp ;
  ns2:body (
   _:genid468
   _:genid470
   _:genid472
 ) ;
  ns2:head (
   _:genid474
   _:genid476
 ) .

_:genid468
  a ns2:ClassAtom ;
  ns2:classPredicate ns0:Technology ;
  ns2:argument1 ns0:Deep_learning_algorithm .

_:genid470
  a ns2:IndividualPropertyAtom ;
  ns2:propertyPredicate ns0:hasTool ;
  ns2:argument1 <https://w3id.org/iot-tta/IoT-WG/ontologies/2022/3/IIoT#x> ;
  ns2:argument2 <https://w3id.org/iot-tta/IoT-WG/ontologies/2022/3/IIoT#y> .

_:genid472
  a ns2:IndividualPropertyAtom ;
  ns2:propertyPredicate ns0:isToolFor ;
  ns2:argument1 <https://w3id.org/iot-tta/IoT-WG/ontologies/2022/3/IIoT#z> ;
  ns2:argument2 <https://w3id.org/iot-tta/IoT-WG/ontologies/2022/3/IIoT#x> .

_:genid474
  a ns2:IndividualPropertyAtom ;
  ns2:propertyPredicate ns0:hasTool ;
  ns2:argument1 <https://w3id.org/iot-tta/IoT-WG/ontologies/2022/3/IIoT#x> ;
  ns2:argument2 <https://w3id.org/iot-tta/IoT-WG/ontologies/2022/3/IIoT#z> .

_:genid476
  a ns2:IndividualPropertyAtom ;
  ns2:propertyPredicate ns0:isToolFor ;
  ns2:argument1 <https://w3id.org/iot-tta/IoT-WG/ontologies/2022/3/IIoT#y> ;
  ns2:argument2 <https://w3id.org/iot-tta/IoT-WG/ontologies/2022/3/IIoT#x> .

[]
  ns1:isRuleEnabled true ;
  rdfs:comment ""@en ;
  rdfs:label "R1s2"@en ;
  a ns2:Imp ;
  ns2:body (
   _:genid479
   _:genid481
   _:genid483
 ) ;
  ns2:head ( _:genid485 ) .

_:genid479
  a ns2:ClassAtom ;
  ns2:classPredicate ns0:Technology ;
  ns2:argument1 ns0:Deep_learning_algorithm .

_:genid481
  a ns2:IndividualPropertyAtom ;
  ns2:propertyPredicate ns0:hasTool ;
  ns2:argument1 <https://w3id.org/iot-tta/IoT-WG/ontologies/2022/3/IIoT#x> ;
  ns2:argument2 <https://w3id.org/iot-tta/IoT-WG/ontologies/2022/3/IIoT#y> .

_:genid483
  a ns2:IndividualPropertyAtom ;
  ns2:propertyPredicate ns0:isToolFor ;
  ns2:argument1 <https://w3id.org/iot-tta/IoT-WG/ontologies/2022/3/IIoT#z> ;
  ns2:argument2 <https://w3id.org/iot-tta/IoT-WG/ontologies/2022/3/IIoT#x> .

_:genid485
  a ns2:BuiltinAtom ;
  ns2:builtin <http://sqwrl.stanford.edu/ontologies/built-ins/3.4/sqwrl.owl#select> ;
  ns2:arguments (
   <https://w3id.org/iot-tta/IoT-WG/ontologies/2022/3/IIoT#x>
   <https://w3id.org/iot-tta/IoT-WG/ontologies/2022/3/IIoT#y>
   <https://w3id.org/iot-tta/IoT-WG/ontologies/2022/3/IIoT#z>
 ) .

[]
  ns1:isRuleEnabled true ;
  rdfs:comment ""@en ;
  rdfs:label "R1sb"@en ;
  a ns2:Imp ;
  ns2:body (
   _:genid491
   _:genid493
 ) ;
  ns2:head ( _:genid495 ) .

_:genid491
  a ns2:ClassAtom ;
  ns2:classPredicate ns0:Technology ;
  ns2:argument1 ns0:Deep_learning_algorithm .

_:genid493
  a ns2:IndividualPropertyAtom ;
  ns2:propertyPredicate ns0:hasTool ;
  ns2:argument1 ns0:Deep_learning_algorithm ;
  ns2:argument2 <https://w3id.org/iot-tta/IoT-WG/ontologies/2022/3/IIoT#y> .

_:genid495
  a ns2:BuiltinAtom ;
  ns2:builtin <http://sqwrl.stanford.edu/ontologies/built-ins/3.4/sqwrl.owl#select> ;
  ns2:arguments ( <https://w3id.org/iot-tta/IoT-WG/ontologies/2022/3/IIoT#y> ) .

[]
  ns1:isRuleEnabled true ;
  rdfs:comment ""@en ;
  rdfs:label "R3sa"@en ;
  a ns2:Imp ;
  ns2:body (
   _:genid499
   _:genid501
   _:genid503
 ) ;
  ns2:head (
   _:genid505
   _:genid507
 ) .

_:genid499
  a ns2:ClassAtom ;
  ns2:classPredicate ns0:Tool ;
  ns2:argument1 ns0:Hadoop .

_:genid501
  a ns2:IndividualPropertyAtom ;
  ns2:propertyPredicate ns0:isApplied ;
  ns2:argument1 <https://w3id.org/iot-tta/IoT-WG/ontologies/2022/3/IIoT#z> ;
  ns2:argument2 <https://w3id.org/iot-tta/IoT-WG/ontologies/2022/3/IIoT#y> .

_:genid503
  a ns2:IndividualPropertyAtom ;
  ns2:propertyPredicate ns0:isUsedBy ;
  ns2:argument1 <https://w3id.org/iot-tta/IoT-WG/ontologies/2022/3/IIoT#x> ;
  ns2:argument2 <https://w3id.org/iot-tta/IoT-WG/ontologies/2022/3/IIoT#y> .

_:genid505
  a ns2:IndividualPropertyAtom ;
  ns2:propertyPredicate ns0:useProgramming ;
  ns2:argument1 <https://w3id.org/iot-tta/IoT-WG/ontologies/2022/3/IIoT#x> ;
  ns2:argument2 <https://w3id.org/iot-tta/IoT-WG/ontologies/2022/3/IIoT#z> .

_:genid507
  a ns2:IndividualPropertyAtom ;
  ns2:propertyPredicate ns0:isToolFor ;
  ns2:argument1 <https://w3id.org/iot-tta/IoT-WG/ontologies/2022/3/IIoT#x> ;
  ns2:argument2 <https://w3id.org/iot-tta/IoT-WG/ontologies/2022/3/IIoT#y> .
